src/dvspec/dafny/att_spec_proofs/dvn_next_invs_19_26.dfy
@@ -5,13 +5,13 @@ include "../specification/network.dfy"
 include "../specification/dvn.dfy"
 include "../att_spec_proofs/inv.dfy"
 include "../att_spec_proofs/assump.dfy"
-include "../att_spec_proofs/fnc_inv.dfy"
+include "../att_spec_proofs/fnc_invs_1_26.dfy"
 include "../att_spec_proofs/helper_sets_lemmas.dfy"
 include "../att_spec_proofs/proofs_intermediate_steps.dfy"
 include "../att_spec_proofs/dvn_next_invs_1_7.dfy"
 include "../att_spec_proofs/dvn_next_invs_8_18.dfy"
 
-module DVN_Next_Invs_19
+module DVN_Next_Invs_19_26
 {
     import opened Types 
     import opened CommonFunctions
@@ -21,7 +21,7 @@ module DVN_Next_Invs_19
     import opened DV
     import opened Att_Inv_With_Empty_Initial_Attestation_Slashing_DB
     import opened Att_Assumptions
-    import opened Fnc_Inv
+    import opened Fnc_Invs_1_26
     import opened Helper_Sets_Lemmas
     import opened Proofs_Intermediate_Steps
     import opened DVN_Next_Invs_1_7
@@ -311,7 +311,6 @@ module DVN_Next_Invs_19
     )    
     requires NextEvent(dvn, event, dvn')  
     requires inv5(dvn)
-    requires inv25(dvn)
     requires inv26(dvn)  
     ensures inv26(dvn')
     {        
@@ -325,7 +324,6 @@ module DVN_Next_Invs_19
                 {
                     case ServeAttstationDuty(attestation_duty) =>   
                         assert inv5_body(dvc);
-                        assert inv25_body(dvc);   
                         assert inv26_body(dvc);                                           
                         lemma_inv26_f_serve_attestation_duty(dvc, attestation_duty, dvc');
                         assert inv26_body(dvc');
@@ -356,6 +354,7 @@ module DVN_Next_Invs_19
             case AdeversaryTakingStep(node, new_attestation_share_sent, messagesReceivedByTheNode) =>
                 
         }   
-    }
+    } 
+
 }   
         
