src/dvspec/dafny/att_spec_proofs/dvn_next_invs_27.dfy
@@ -1,0 +1,343 @@
+include "../commons.dfy"
+include "../specification/dvc_spec.dfy"
+include "../specification/consensus.dfy"
+include "../specification/network.dfy"
+include "../specification/dvn.dfy"
+include "../att_spec_proofs/inv.dfy"
+include "../att_spec_proofs/assump.dfy"
+include "../att_spec_proofs/fnc_invs_1_26.dfy"
+include "../att_spec_proofs/helper_sets_lemmas.dfy"
+include "../att_spec_proofs/proofs_intermediate_steps.dfy"
+include "../att_spec_proofs/dvn_next_invs_1_7.dfy"
+include "../att_spec_proofs/dvn_next_invs_8_18.dfy"
+include "../att_spec_proofs/dvn_next_invs_19_26.dfy"
+include "../att_spec_proofs/fnc_invs_27.dfy"
+
+module DVN_Next_Invs_27
+{
+    import opened Types 
+    import opened CommonFunctions
+    import opened ConsensusSpec
+    import opened NetworkSpec
+    import opened DVCNode_Spec
+    import opened DV
+    import opened Att_Inv_With_Empty_Initial_Attestation_Slashing_DB
+    import opened Att_Assumptions
+    import opened Fnc_Invs_1_26
+    import opened Helper_Sets_Lemmas
+    import opened Proofs_Intermediate_Steps
+    import opened DVN_Next_Invs_1_7
+    import opened DVN_Next_Invs_8_18
+    import opened DVN_Next_Invs_19_26
+    import opened Fnc_Invs_27
+    
+
+    lemma lemma_inv27_dvn_next(
+        dvn: DVState,
+        event: DV.Event,
+        dvn': DVState
+    )    
+    requires NextEvent(dvn, event, dvn')  
+    requires inv5(dvn)
+    requires inv25(dvn)
+    requires inv27(dvn)  
+    ensures inv27(dvn')
+    {        
+        match event 
+        {
+            case HonestNodeTakingStep(node, nodeEvent, nodeOutputs) =>
+                var dvc := dvn.honest_nodes_states[node];
+                var dvc' := dvn'.honest_nodes_states[node];                
+                
+                match nodeEvent
+                {
+                    case ServeAttstationDuty(attestation_duty) =>   
+                        assert inv5_body(dvc);
+                        assert inv25_body(dvc);   
+                        assert inv27_body(dvc);                                           
+                        lemma_inv27_f_serve_attestation_duty(dvc, attestation_duty, dvc');
+                        assert inv27_body(dvc');
+                        
+                    case AttConsensusDecided(id, decided_attestation_data) => 
+                        lemma_inv27_f_att_consensus_decided(dvc, id, decided_attestation_data, dvc');
+                        assert inv27_body(dvc');
+                        
+                    case ReceviedAttesttionShare(attestation_share) =>                         
+                        lemma_inv27_f_listen_for_attestation_shares(dvc, attestation_share, dvc');
+                        assert inv27_body(dvc');
+                       
+                    case ImportedNewBlock(block) => 
+                        var dvc_mod := add_block_to_bn(dvc, block);
+                        lemma_inv5_add_block_to_bn(dvc, block, dvc_mod);
+                        assert inv5_body(dvc_mod);
+                        lemma_inv27_add_block_to_bn(dvc, block, dvc_mod);
+                        assert inv27_body(dvc_mod);
+                        lemma_inv27_f_listen_for_new_imported_blocks(dvc_mod, block, dvc');                        
+                        assert inv27_body(dvc');
+
+                    case ResendAttestationShares =>                                                                      
+
+                    case NoEvent => 
+                        
+                }
+                
+            case AdeversaryTakingStep(node, new_attestation_share_sent, messagesReceivedByTheNode) =>
+                
+        }   
+    }
+
+    lemma lemma_inv28_dvn_next(
+        dvn: DVState,
+        event: DV.Event,
+        dvn': DVState
+    )    
+    requires NextEvent(dvn, event, dvn')  
+    requires inv5(dvn)
+    requires inv26(dvn)
+    requires inv28(dvn)  
+    ensures inv28(dvn')
+    {        
+        match event 
+        {
+            case HonestNodeTakingStep(node, nodeEvent, nodeOutputs) =>
+                var dvc := dvn.honest_nodes_states[node];
+                var dvc' := dvn'.honest_nodes_states[node];                
+                
+                match nodeEvent
+                {
+                    case ServeAttstationDuty(attestation_duty) =>   
+                        assert inv5_body(dvc);
+                        assert inv26_body(dvc);   
+                        assert inv28_body(dvc);                                           
+                        lemma_inv28_f_serve_attestation_duty(dvc, attestation_duty, dvc');
+                        assert inv28_body(dvc');
+                        
+                    case AttConsensusDecided(id, decided_attestation_data) => 
+                        lemma_inv28_f_att_consensus_decided(dvc, id, decided_attestation_data, dvc');
+                        assert inv28_body(dvc');
+                        
+                    case ReceviedAttesttionShare(attestation_share) =>                         
+                        lemma_inv28_f_listen_for_attestation_shares(dvc, attestation_share, dvc');
+                        assert inv28_body(dvc');
+                       
+                    case ImportedNewBlock(block) => 
+                        var dvc_mod := add_block_to_bn(dvc, block);
+                        lemma_inv5_add_block_to_bn(dvc, block, dvc_mod);
+                        assert inv5_body(dvc_mod);
+                        lemma_inv28_add_block_to_bn(dvc, block, dvc_mod);
+                        assert inv28_body(dvc_mod);
+                        lemma_inv28_f_listen_for_new_imported_blocks(dvc_mod, block, dvc');                        
+                        assert inv28_body(dvc');
+
+                    case ResendAttestationShares =>                                                                      
+
+                    case NoEvent => 
+                        
+                }
+                
+            case AdeversaryTakingStep(node, new_attestation_share_sent, messagesReceivedByTheNode) =>
+                
+        }   
+    }
+
+    lemma lemma_inv29_dvn_next(
+        dvn: DVState,
+        event: DV.Event,
+        dvn': DVState
+    )    
+    requires NextEvent(dvn, event, dvn')  
+    requires inv5(dvn)
+    requires inv25(dvn)
+    requires inv29(dvn)  
+    ensures inv29(dvn')
+    {        
+        match event 
+        {
+            case HonestNodeTakingStep(node, nodeEvent, nodeOutputs) =>
+                var dvc := dvn.honest_nodes_states[node];
+                var dvc' := dvn'.honest_nodes_states[node];                
+                
+                match nodeEvent
+                {
+                    case ServeAttstationDuty(attestation_duty) =>   
+                        assert inv5_body(dvc);
+                        assert inv25_body(dvc);   
+                        assert inv29_body(dvc);                                           
+                        lemma_inv29_f_serve_attestation_duty(dvc, attestation_duty, dvc');
+                        assert inv29_body(dvc');
+                        
+                    case AttConsensusDecided(id, decided_attestation_data) => 
+                        lemma_inv29_f_att_consensus_decided(dvc, id, decided_attestation_data, dvc');
+                        assert inv29_body(dvc');
+                        
+                    case ReceviedAttesttionShare(attestation_share) =>                         
+                        lemma_inv29_f_listen_for_attestation_shares(dvc, attestation_share, dvc');
+                        assert inv29_body(dvc');
+                       
+                    case ImportedNewBlock(block) => 
+                        var dvc_mod := add_block_to_bn(dvc, block);
+                        lemma_inv5_add_block_to_bn(dvc, block, dvc_mod);
+                        assert inv5_body(dvc_mod);
+                        lemma_inv29_add_block_to_bn(dvc, block, dvc_mod);
+                        assert inv29_body(dvc_mod);
+                        lemma_inv29_f_listen_for_new_imported_blocks(dvc_mod, block, dvc');                        
+                        assert inv29_body(dvc');
+
+                    case ResendAttestationShares =>                                                                      
+
+                    case NoEvent => 
+                        
+                }
+                
+            case AdeversaryTakingStep(node, new_attestation_share_sent, messagesReceivedByTheNode) =>
+                
+        }   
+    }
+
+    lemma lemma_inv30_dvn_next(
+        dvn: DVState,
+        event: DV.Event,
+        dvn': DVState
+    )    
+    requires NextEvent(dvn, event, dvn')  
+    ensures inv30(dvn, event, dvn')
+    {        
+        match event 
+        {
+            case HonestNodeTakingStep(node, nodeEvent, nodeOutputs) =>
+                var dvc := dvn.honest_nodes_states[node];
+                var dvc' := dvn'.honest_nodes_states[node];                
+                
+                match nodeEvent
+                {
+                    case ServeAttstationDuty(attestation_duty) =>   
+                        lemma_inv30_f_serve_attestation_duty(dvc, attestation_duty, dvc');
+                        assert inv30_body(dvc, dvc');
+                        
+                    case AttConsensusDecided(id, decided_attestation_data) => 
+                        lemma_inv30_f_att_consensus_decided(dvc, id, decided_attestation_data, dvc');
+                        assert inv30_body(dvc, dvc');
+                        
+                    case ReceviedAttesttionShare(attestation_share) =>                         
+                        lemma_inv30_f_listen_for_attestation_shares(dvc, attestation_share, dvc');
+                        assert inv30_body(dvc, dvc');
+                       
+                    case ImportedNewBlock(block) => 
+                        var dvc_mod := add_block_to_bn(dvc, block);
+                        lemma_inv30_add_block_to_bn(dvc, block, dvc_mod);
+                        assert inv30_body(dvc, dvc_mod);
+                        lemma_inv30_f_listen_for_new_imported_blocks(dvc_mod, block, dvc');                        
+                        assert inv30_body(dvc_mod, dvc');
+
+                    case ResendAttestationShares =>                                                                      
+
+                    case NoEvent => 
+                        
+                }
+                
+            case AdeversaryTakingStep(node, new_attestation_share_sent, messagesReceivedByTheNode) =>
+                
+        }   
+    }
+
+    lemma lemma_inv31_dvn_next(
+        dvn: DVState,
+        event: DV.Event,
+        dvn': DVState
+    )    
+    requires NextEvent(dvn, event, dvn')  
+    requires inv5(dvn)
+    requires inv26(dvn)
+    requires inv31(dvn)  
+    ensures inv31(dvn')
+    {        
+        match event 
+        {
+            case HonestNodeTakingStep(node, nodeEvent, nodeOutputs) =>
+                var dvc := dvn.honest_nodes_states[node];
+                var dvc' := dvn'.honest_nodes_states[node];                
+                
+                match nodeEvent
+                {
+                    case ServeAttstationDuty(attestation_duty) =>   
+                        assert inv5_body(dvc);
+                        assert inv26_body(dvc);   
+                        assert inv31_body(dvc);                                           
+                        lemma_inv31_f_serve_attestation_duty(dvc, attestation_duty, dvc');
+                        assert inv31_body(dvc');
+                        
+                    case AttConsensusDecided(id, decided_attestation_data) => 
+                        lemma_inv31_f_att_consensus_decided(dvc, id, decided_attestation_data, dvc');
+                        assert inv31_body(dvc');
+                        
+                    case ReceviedAttesttionShare(attestation_share) =>                         
+                        lemma_inv31_f_listen_for_attestation_shares(dvc, attestation_share, dvc');
+                        assert inv31_body(dvc');
+                       
+                    case ImportedNewBlock(block) => 
+                        var dvc_mod := add_block_to_bn(dvc, block);
+                        lemma_inv5_add_block_to_bn(dvc, block, dvc_mod);
+                        assert inv5_body(dvc_mod);
+                        lemma_inv31_add_block_to_bn(dvc, block, dvc_mod);
+                        assert inv31_body(dvc_mod);
+                        lemma_inv31_f_listen_for_new_imported_blocks(dvc_mod, block, dvc');                        
+                        assert inv31_body(dvc');
+
+                    case ResendAttestationShares =>                                                                      
+
+                    case NoEvent => 
+                        
+                }
+                
+            case AdeversaryTakingStep(node, new_attestation_share_sent, messagesReceivedByTheNode) =>
+                
+        }   
+    }
+
+    lemma lemma_inv32_dvn_next(
+        dvn: DVState,
+        event: DV.Event,
+        dvn': DVState
+    )    
+    requires NextEvent(dvn, event, dvn')  
+    ensures inv32(dvn, event, dvn')
+    {        
+        match event 
+        {
+            case HonestNodeTakingStep(node, nodeEvent, nodeOutputs) =>
+                var dvc := dvn.honest_nodes_states[node];
+                var dvc' := dvn'.honest_nodes_states[node];                
+                
+                match nodeEvent
+                {
+                    case ServeAttstationDuty(attestation_duty) =>   
+                        lemma_inv32_f_serve_attestation_duty(dvc, attestation_duty, dvc');
+                        assert inv32_body(dvc, dvc');
+                        
+                    case AttConsensusDecided(id, decided_attestation_data) => 
+                        lemma_inv32_f_att_consensus_decided(dvc, id, decided_attestation_data, dvc');
+                        assert inv32_body(dvc, dvc');
+                        
+                    case ReceviedAttesttionShare(attestation_share) =>                         
+                        lemma_inv32_f_listen_for_attestation_shares(dvc, attestation_share, dvc');
+                        assert inv32_body(dvc, dvc');
+                       
+                    case ImportedNewBlock(block) => 
+                        var dvc_mod := add_block_to_bn(dvc, block);
+                        lemma_inv32_add_block_to_bn(dvc, block, dvc_mod);
+                        assert inv32_body(dvc, dvc_mod);
+                        lemma_inv32_f_listen_for_new_imported_blocks(dvc_mod, block, dvc');                        
+                        assert inv32_body(dvc_mod, dvc');
+
+                    case ResendAttestationShares =>                                                                      
+
+                    case NoEvent => 
+                        
+                }
+                
+            case AdeversaryTakingStep(node, new_attestation_share_sent, messagesReceivedByTheNode) =>
+                
+        }   
+    }
+}   
+        
