src/dvspec/dafny/att_spec_proofs/dvn_next_invs_8_18.dfy
@@ -5,7 +5,7 @@ include "../specification/network.dfy"
 include "../specification/dvn.dfy"
 include "../att_spec_proofs/inv.dfy"
 include "../att_spec_proofs/assump.dfy"
-include "../att_spec_proofs/fnc_inv.dfy"
+include "../att_spec_proofs/fnc_invs_1_26.dfy"
 include "../att_spec_proofs/helper_sets_lemmas.dfy"
 include "../att_spec_proofs/proofs_intermediate_steps.dfy"
 include "../att_spec_proofs/dvn_next_invs_1_7.dfy"
@@ -20,7 +20,7 @@ module DVN_Next_Invs_8_18
     import opened DV
     import opened Att_Inv_With_Empty_Initial_Attestation_Slashing_DB
     import opened Att_Assumptions
-    import opened Fnc_Inv
+    import opened Fnc_Invs_1_26
     import opened Helper_Sets_Lemmas
     import opened Proofs_Intermediate_Steps
     import opened DVN_Next_Invs_1_7
@@ -167,8 +167,10 @@ module DVN_Next_Invs_8_18
     )    
     requires NextEvent(dvn, event, dvn')    
     requires inv13(dvn)
-    ensures inv13(dvn)
-    { }
+    ensures inv13(dvn')
+    { 
+        assert dvn.sequence_attestation_duties_to_be_served == dvn'.sequence_attestation_duties_to_be_served;
+    }
     
 
     // It takes more than 60 seconds to prove lemma_inv16_dvn_next.
