src/dvspec/dafny/att_spec_proofs/fnc_invs_27.dfy
@@ -1,0 +1,1876 @@
+include "../commons.dfy"
+include "../specification/dvc_spec.dfy"
+include "../specification/consensus.dfy"
+include "../specification/network.dfy"
+include "../specification/dvn.dfy"
+include "../att_spec_proofs/inv.dfy"
+include "../att_spec_proofs/assump.dfy"
+include "../att_spec_proofs/helper_sets_lemmas.dfy"
+include "../att_spec_proofs/common_proofs.dfy"
+include "../att_spec_proofs/fnc_invs_1_26.dfy"
+
+module Fnc_Invs_27
+{
+    import opened Types 
+    import opened CommonFunctions
+    import opened ConsensusSpec
+    import opened NetworkSpec
+    import opened DVCNode_Spec
+    import opened DV
+    import opened Att_Inv_With_Empty_Initial_Attestation_Slashing_DB
+    import opened Att_Assumptions
+    import opened Helper_Sets_Lemmas
+    import opened Common_Proofs
+    import opened Fnc_Invs_1_26
+    
+    
+    
+
+    lemma lemma_inv27_add_block_to_bn(
+        s: DVCNodeState,
+        block: BeaconBlock,
+        s': DVCNodeState 
+    )
+    requires add_block_to_bn.requires(s, block)
+    requires s' == add_block_to_bn(s, block)    
+    requires inv27_body(s)
+    ensures inv27_body(s')
+    { }
+
+    lemma lemma_inv27_f_listen_for_attestation_shares(
+        process: DVCNodeState,
+        attestation_share: AttestationShare,
+        process': DVCNodeState
+    )
+    requires f_listen_for_attestation_shares.requires(process, attestation_share)
+    requires process' == f_listen_for_attestation_shares(process, attestation_share).state        
+    requires inv27_body(process)
+    ensures inv27_body(process')
+    { }
+
+    lemma lemma_inv27_f_start_next_duty(process: DVCNodeState, attestation_duty: AttestationDuty, process': DVCNodeState)
+    requires f_start_next_duty.requires(process, attestation_duty)
+    requires process' == f_start_next_duty(process, attestation_duty).state   
+    requires attestation_duty in process.all_rcvd_duties
+    requires inv27_body(process)
+    ensures inv27_body(process')
+    { } 
+
+    lemma lemma_inv27_f_resend_attestation_share(
+        process: DVCNodeState,
+        process': DVCNodeState)
+    requires f_resend_attestation_share.requires(process)
+    requires process' == f_resend_attestation_share(process).state        
+    requires inv27_body(process)
+    ensures inv27_body(process')
+    { } 
+
+    
+
+    lemma lemma_inv27_f_check_for_next_queued_duty(
+        process: DVCNodeState,
+        process': DVCNodeState
+    )
+    requires f_check_for_next_queued_duty.requires(process)
+    requires process' == f_check_for_next_queued_duty(process).state    
+    requires inv5_body(process)
+    requires inv25_body(process)
+    requires inv27_body(process)
+    ensures inv27_body(process')
+    decreases process.attestation_duties_queue
+    {
+        if  && process.attestation_duties_queue != [] 
+            && (
+                || process.attestation_duties_queue[0].slot in process.future_att_consensus_instances_already_decided
+                || !process.current_attestation_duty.isPresent()
+            )    
+        {            
+                if process.attestation_duties_queue[0].slot in process.future_att_consensus_instances_already_decided.Keys 
+                {
+                    var queue_head := process.attestation_duties_queue[0];
+                    var new_attestation_slashing_db := f_update_attestation_slashing_db(process.attestation_slashing_db, process.future_att_consensus_instances_already_decided[queue_head.slot]);
+                    var process_mod := process.(
+                        attestation_duties_queue := process.attestation_duties_queue[1..],
+                        future_att_consensus_instances_already_decided := process.future_att_consensus_instances_already_decided - {queue_head.slot},
+                        attestation_slashing_db := new_attestation_slashing_db,
+                        attestation_consensus_engine_state := updateConsensusInstanceValidityCheck(
+                            process.attestation_consensus_engine_state,
+                            new_attestation_slashing_db
+                        )                        
+                    );
+
+                    lemma_updateConsensusInstanceValidityCheck(
+                                process.attestation_consensus_engine_state,
+                                new_attestation_slashing_db,
+                                process_mod.attestation_consensus_engine_state 
+                                );
+
+                    assert process_mod.attestation_consensus_engine_state.att_slashing_db_hist.Keys
+                                == process.attestation_consensus_engine_state.att_slashing_db_hist.Keys 
+                                        + process.attestation_consensus_engine_state.attestation_consensus_active_instances.Keys;
+
+                    assert inv25_body(process_mod);
+
+                    assert inv5_body(process_mod);
+                    assert inv27_body(process_mod);
+                    lemma_inv27_f_check_for_next_queued_duty(process_mod, process');
+                }
+                else
+                { 
+                    var process_mod := process.(
+                        attestation_duties_queue := process.attestation_duties_queue[1..]
+                    );     
+                    assert inv5_body(process_mod);
+                    assert inv27_body(process_mod);
+                    lemma_inv27_f_start_next_duty(process_mod, process.attestation_duties_queue[0], process');
+                }
+        }
+        else
+        { 
+            assert process'.all_rcvd_duties == process.all_rcvd_duties;
+        }
+    }
+
+    
+
+    lemma lemma_inv27_f_att_consensus_decided(
+        process: DVCNodeState,
+        id: Slot,
+        decided_attestation_data: AttestationData, 
+        process': DVCNodeState
+    )
+    requires f_att_consensus_decided.requires(process, id, decided_attestation_data)
+    requires process' == f_att_consensus_decided(process, id, decided_attestation_data).state         
+    requires inv5_body(process)
+    requires inv25_body(process)
+    requires inv27_body(process)
+    ensures inv27_body(process')
+    {
+        
+        var local_current_attestation_duty := process.current_attestation_duty.safe_get();
+        var attestation_slashing_db := f_update_attestation_slashing_db(process.attestation_slashing_db, decided_attestation_data);
+
+        var fork_version := bn_get_fork_version(compute_start_slot_at_epoch(decided_attestation_data.target.epoch));
+        var attestation_signing_root := compute_attestation_signing_root(decided_attestation_data, fork_version);
+        var attestation_signature_share := rs_sign_attestation(decided_attestation_data, fork_version, attestation_signing_root, process.rs);
+        var attestation_with_signature_share := AttestationShare(
+                aggregation_bits := get_aggregation_bits(local_current_attestation_duty.validator_index),
+                data := decided_attestation_data, 
+                signature := attestation_signature_share
+            ); 
+
+        var new_attestation_consensus_engine_state := updateConsensusInstanceValidityCheck(
+                                                            process.attestation_consensus_engine_state,
+                                                            attestation_slashing_db
+                                                      );
+
+        var process_mod := 
+            process.(
+                current_attestation_duty := None,
+                attestation_shares_to_broadcast := process.attestation_shares_to_broadcast[local_current_attestation_duty.slot := attestation_with_signature_share],
+                attestation_slashing_db := attestation_slashing_db,
+                attestation_consensus_engine_state := new_attestation_consensus_engine_state
+            );
+    
+        lemma_updateConsensusInstanceValidityCheck(
+                                process.attestation_consensus_engine_state,
+                                attestation_slashing_db,
+                                process_mod.attestation_consensus_engine_state 
+                                );
+
+        assert process_mod.attestation_consensus_engine_state.att_slashing_db_hist.Keys
+                    == process.attestation_consensus_engine_state.att_slashing_db_hist.Keys 
+                            + process.attestation_consensus_engine_state.attestation_consensus_active_instances.Keys;
+
+
+        assert inv5_body(process_mod);
+        assert inv25_body(process_mod);
+
+        assert inv27_body(process_mod);
+
+        var ret_dvc := f_check_for_next_queued_duty(process_mod).state;
+        lemma_inv5_f_check_for_next_queued_duty(process_mod, ret_dvc);
+        assert inv5_body(ret_dvc);
+        
+        lemma_inv27_f_check_for_next_queued_duty(process_mod, ret_dvc);
+        assert inv27_body(ret_dvc);
+
+        assert process' == ret_dvc;        
+    }
+
+    lemma lemma_inv27_f_serve_attestation_duty(
+        process: DVCNodeState,
+        attestation_duty: AttestationDuty,
+        process': DVCNodeState
+    )  
+    requires f_serve_attestation_duty.requires(process, attestation_duty)
+    requires process' == f_serve_attestation_duty(process, attestation_duty).state
+    requires inv5_body(process)
+    requires inv25_body(process)
+    requires inv27_body(process)
+    ensures inv27_body(process')
+    {
+        var process_mod := process.(
+                attestation_duties_queue := process.attestation_duties_queue + [attestation_duty],
+                all_rcvd_duties := process.all_rcvd_duties + {attestation_duty}
+            );        
+
+        assert inv5_body(process_mod);
+        assert inv25_body(process_mod);
+        assert inv27_body(process_mod);
+        
+        lemma_inv27_f_check_for_next_queued_duty(process_mod, process');        
+    }
+
+    lemma lemma_inv27_f_listen_for_new_imported_blocks(
+        process: DVCNodeState,
+        block: BeaconBlock,
+        process': DVCNodeState
+    )
+    requires f_listen_for_new_imported_blocks.requires(process, block)
+    requires process' == f_listen_for_new_imported_blocks(process, block).state        
+    requires inv5_body(process)
+    requires inv25_body(process)
+    requires inv27_body(process)
+    ensures inv27_body(process')
+    {
+        var new_consensus_instances_already_decided := f_listen_for_new_imported_blocks_helper_1(process, block);
+
+        var att_consensus_instances_already_decided := process.future_att_consensus_instances_already_decided + new_consensus_instances_already_decided;
+
+        var future_att_consensus_instances_already_decided := 
+            f_listen_for_new_imported_blocks_helper_2(process, att_consensus_instances_already_decided);
+
+        var process :=
+                process.(
+                    future_att_consensus_instances_already_decided := future_att_consensus_instances_already_decided,
+                    attestation_consensus_engine_state := stopConsensusInstances(
+                                    process.attestation_consensus_engine_state,
+                                    att_consensus_instances_already_decided.Keys
+                    ),
+                    attestation_shares_to_broadcast := process.attestation_shares_to_broadcast - att_consensus_instances_already_decided.Keys,
+                    rcvd_attestation_shares := process.rcvd_attestation_shares - att_consensus_instances_already_decided.Keys                    
+                );    
+        
+        assert inv5_body(process);
+        assert inv25_body(process);
+        assert inv27_body(process);
+
+        if process.current_attestation_duty.isPresent() && process.current_attestation_duty.safe_get().slot in att_consensus_instances_already_decided
+        {
+            var decided_attestation_data := att_consensus_instances_already_decided[process.current_attestation_duty.safe_get().slot];
+            var new_attestation_slashing_db := f_update_attestation_slashing_db(process.attestation_slashing_db, decided_attestation_data);
+            var new_attestation_consensus_engine_state := updateConsensusInstanceValidityCheck(
+                                                            process.attestation_consensus_engine_state,
+                                                            new_attestation_slashing_db
+                                                          );  
+            var process_mod := process.(
+                current_attestation_duty := None,
+                attestation_slashing_db := new_attestation_slashing_db,
+                attestation_consensus_engine_state := new_attestation_consensus_engine_state
+            );
+
+            lemma_updateConsensusInstanceValidityCheck(
+                                process.attestation_consensus_engine_state,
+                                new_attestation_slashing_db,
+                                process_mod.attestation_consensus_engine_state 
+                                );
+
+            assert process_mod.attestation_consensus_engine_state.att_slashing_db_hist.Keys
+                    == process.attestation_consensus_engine_state.att_slashing_db_hist.Keys 
+                            + process.attestation_consensus_engine_state.attestation_consensus_active_instances.Keys;
+
+            
+            assert inv5_body(process_mod);
+            assert inv25_body(process_mod);
+            assert inv27_body(process_mod);
+
+            lemma_inv27_f_check_for_next_queued_duty(process_mod, process');
+        }
+        else
+        {               
+            assert inv27_body(process);
+        }
+    }  
+
+    
+    lemma lemma_inv28_add_block_to_bn(
+        s: DVCNodeState,
+        block: BeaconBlock,
+        s': DVCNodeState 
+    )
+    requires add_block_to_bn.requires(s, block)
+    requires s' == add_block_to_bn(s, block)    
+    requires inv28_body(s)
+    ensures inv28_body(s')
+    { }
+
+    lemma lemma_inv28_f_listen_for_attestation_shares(
+        process: DVCNodeState,
+        attestation_share: AttestationShare,
+        process': DVCNodeState
+    )
+    requires f_listen_for_attestation_shares.requires(process, attestation_share)
+    requires process' == f_listen_for_attestation_shares(process, attestation_share).state        
+    requires inv28_body(process)
+    ensures inv28_body(process')
+    { }
+
+    lemma lemma_inv28_f_start_next_duty(process: DVCNodeState, attestation_duty: AttestationDuty, process': DVCNodeState)
+    requires f_start_next_duty.requires(process, attestation_duty)
+    requires process' == f_start_next_duty(process, attestation_duty).state   
+    requires attestation_duty in process.all_rcvd_duties
+    requires inv28_body(process)
+    ensures inv28_body(process')
+    { } 
+
+    lemma lemma_inv28_f_resend_attestation_share(
+        process: DVCNodeState,
+        process': DVCNodeState)
+    requires f_resend_attestation_share.requires(process)
+    requires process' == f_resend_attestation_share(process).state        
+    requires inv28_body(process)
+    ensures inv28_body(process')
+    { } 
+
+    lemma lemma_inv28_f_check_for_next_queued_duty(
+        process: DVCNodeState,
+        process': DVCNodeState
+    )
+    requires f_check_for_next_queued_duty.requires(process)
+    requires process' == f_check_for_next_queued_duty(process).state    
+    requires inv5_body(process)
+    requires inv26_body(process)
+    requires inv28_body(process)
+    ensures inv28_body(process')
+    decreases process.attestation_duties_queue
+    {
+        if  && process.attestation_duties_queue != [] 
+            && (
+                || process.attestation_duties_queue[0].slot in process.future_att_consensus_instances_already_decided
+                || !process.current_attestation_duty.isPresent()
+            )    
+        {            
+                if process.attestation_duties_queue[0].slot in process.future_att_consensus_instances_already_decided.Keys 
+                {
+                    var queue_head := process.attestation_duties_queue[0];
+                    var new_attestation_slashing_db := f_update_attestation_slashing_db(process.attestation_slashing_db, process.future_att_consensus_instances_already_decided[queue_head.slot]);
+                    var new_attestation_consensus_engine_state := updateConsensusInstanceValidityCheck(
+                            process.attestation_consensus_engine_state,
+                            new_attestation_slashing_db
+                        ); 
+
+                    assert inv28_body_ces(process.attestation_consensus_engine_state);
+                    assert new_attestation_consensus_engine_state 
+                                == updateConsensusInstanceValidityCheck(
+                                        process.attestation_consensus_engine_state, 
+                                        new_attestation_slashing_db);
+                    
+                    lemma_inv28_updateConsensusInstanceValidityCheck(
+                        process.attestation_consensus_engine_state,
+                        new_attestation_slashing_db,
+                        new_attestation_consensus_engine_state);
+                    assert inv28_body_ces(new_attestation_consensus_engine_state);
+
+                    var process_mod := process.(
+                        attestation_duties_queue := process.attestation_duties_queue[1..],
+                        future_att_consensus_instances_already_decided := process.future_att_consensus_instances_already_decided - {queue_head.slot},
+                        attestation_slashing_db := new_attestation_slashing_db,
+                        attestation_consensus_engine_state := new_attestation_consensus_engine_state                                              
+                    );
+                    assert inv28_body(process_mod);
+
+                    lemma_updateConsensusInstanceValidityCheck(
+                                process.attestation_consensus_engine_state,
+                                new_attestation_slashing_db,
+                                process_mod.attestation_consensus_engine_state 
+                                );
+
+                    assert process_mod.attestation_consensus_engine_state.att_slashing_db_hist.Keys
+                                == process.attestation_consensus_engine_state.att_slashing_db_hist.Keys 
+                                        + process.attestation_consensus_engine_state.attestation_consensus_active_instances.Keys;
+                    assert inv26_body(process_mod);
+                    assert inv5_body(process_mod);
+
+                    lemma_inv28_f_check_for_next_queued_duty(process_mod, process');
+                    assert inv28_body(process');
+                }
+                else
+                { 
+                    var process_mod := process.(
+                        attestation_duties_queue := process.attestation_duties_queue[1..]
+                    );     
+                    assert inv5_body(process_mod);
+                    assert inv28_body(process_mod);
+                    lemma_inv28_f_start_next_duty(process_mod, process.attestation_duties_queue[0], process');
+                    assert inv28_body(process');
+                }
+        }
+        else
+        { 
+            assert process'.all_rcvd_duties == process.all_rcvd_duties;
+            assert inv28_body(process');
+        }
+    }
+
+    lemma lemma_inv28_f_att_consensus_decided(
+        process: DVCNodeState,
+        id: Slot,
+        decided_attestation_data: AttestationData, 
+        process': DVCNodeState
+    )
+    requires f_att_consensus_decided.requires(process, id, decided_attestation_data)
+    requires process' == f_att_consensus_decided(process, id, decided_attestation_data).state         
+    requires inv5_body(process)
+    requires inv26_body(process)
+    requires inv28_body(process)
+    ensures inv28_body(process')
+    {
+        
+        var local_current_attestation_duty := process.current_attestation_duty.safe_get();
+        var attestation_slashing_db := f_update_attestation_slashing_db(process.attestation_slashing_db, decided_attestation_data);
+
+        var fork_version := bn_get_fork_version(compute_start_slot_at_epoch(decided_attestation_data.target.epoch));
+        var attestation_signing_root := compute_attestation_signing_root(decided_attestation_data, fork_version);
+        var attestation_signature_share := rs_sign_attestation(decided_attestation_data, fork_version, attestation_signing_root, process.rs);
+        var attestation_with_signature_share := AttestationShare(
+                aggregation_bits := get_aggregation_bits(local_current_attestation_duty.validator_index),
+                data := decided_attestation_data, 
+                signature := attestation_signature_share
+            ); 
+
+        var new_attestation_consensus_engine_state := updateConsensusInstanceValidityCheck(
+                                                            process.attestation_consensus_engine_state,
+                                                            attestation_slashing_db
+                                                      );
+
+        var process_mod := 
+            process.(
+                current_attestation_duty := None,
+                attestation_shares_to_broadcast := process.attestation_shares_to_broadcast[local_current_attestation_duty.slot := attestation_with_signature_share],
+                attestation_slashing_db := attestation_slashing_db,
+                attestation_consensus_engine_state := new_attestation_consensus_engine_state
+            );
+    
+        lemma_updateConsensusInstanceValidityCheck(
+                                process.attestation_consensus_engine_state,
+                                attestation_slashing_db,
+                                process_mod.attestation_consensus_engine_state 
+                                );
+
+        assert process_mod.attestation_consensus_engine_state.att_slashing_db_hist.Keys
+                    == process.attestation_consensus_engine_state.att_slashing_db_hist.Keys 
+                            + process.attestation_consensus_engine_state.attestation_consensus_active_instances.Keys;
+
+
+        assert inv5_body(process_mod);
+        assert inv26_body(process_mod);
+
+        assert inv28_body(process_mod);
+
+        var ret_dvc := f_check_for_next_queued_duty(process_mod).state;
+        lemma_inv5_f_check_for_next_queued_duty(process_mod, ret_dvc);
+        assert inv5_body(ret_dvc);
+        
+        lemma_inv28_f_check_for_next_queued_duty(process_mod, ret_dvc);
+        assert inv28_body(ret_dvc);
+
+        assert process' == ret_dvc;        
+    }
+
+    lemma lemma_inv28_f_serve_attestation_duty(
+        process: DVCNodeState,
+        attestation_duty: AttestationDuty,
+        process': DVCNodeState
+    )  
+    requires f_serve_attestation_duty.requires(process, attestation_duty)
+    requires process' == f_serve_attestation_duty(process, attestation_duty).state
+    requires inv5_body(process)
+    requires inv26_body(process)
+    requires inv28_body(process)
+    ensures inv28_body(process')
+    {
+        var process_mod := process.(
+                attestation_duties_queue := process.attestation_duties_queue + [attestation_duty],
+                all_rcvd_duties := process.all_rcvd_duties + {attestation_duty}
+            );        
+
+        assert inv5_body(process_mod);
+        assert inv26_body(process_mod);
+        assert inv28_body(process_mod);
+        
+        lemma_inv28_f_check_for_next_queued_duty(process_mod, process');        
+    }
+
+    lemma lemma_inv28_f_listen_for_new_imported_blocks(
+        process: DVCNodeState,
+        block: BeaconBlock,
+        process': DVCNodeState
+    )
+    requires f_listen_for_new_imported_blocks.requires(process, block)
+    requires process' == f_listen_for_new_imported_blocks(process, block).state        
+    requires inv5_body(process)
+    requires inv26_body(process)
+    requires inv28_body(process)
+    ensures inv28_body(process')
+    {
+        var new_consensus_instances_already_decided := f_listen_for_new_imported_blocks_helper_1(process, block);
+
+        var att_consensus_instances_already_decided := process.future_att_consensus_instances_already_decided + new_consensus_instances_already_decided;
+
+        var future_att_consensus_instances_already_decided := 
+            f_listen_for_new_imported_blocks_helper_2(process, att_consensus_instances_already_decided);
+
+        var process :=
+                process.(
+                    future_att_consensus_instances_already_decided := future_att_consensus_instances_already_decided,
+                    attestation_consensus_engine_state := stopConsensusInstances(
+                                    process.attestation_consensus_engine_state,
+                                    att_consensus_instances_already_decided.Keys
+                    ),
+                    attestation_shares_to_broadcast := process.attestation_shares_to_broadcast - att_consensus_instances_already_decided.Keys,
+                    rcvd_attestation_shares := process.rcvd_attestation_shares - att_consensus_instances_already_decided.Keys                    
+                );    
+        
+        assert inv5_body(process);
+        assert inv26_body(process);
+        assert inv28_body(process);
+
+        if process.current_attestation_duty.isPresent() && process.current_attestation_duty.safe_get().slot in att_consensus_instances_already_decided
+        {
+            var decided_attestation_data := att_consensus_instances_already_decided[process.current_attestation_duty.safe_get().slot];
+            var new_attestation_slashing_db := f_update_attestation_slashing_db(process.attestation_slashing_db, decided_attestation_data);
+            var new_attestation_consensus_engine_state := updateConsensusInstanceValidityCheck(
+                                                            process.attestation_consensus_engine_state,
+                                                            new_attestation_slashing_db
+                                                          );  
+            var process_mod := process.(
+                current_attestation_duty := None,
+                attestation_slashing_db := new_attestation_slashing_db,
+                attestation_consensus_engine_state := new_attestation_consensus_engine_state
+            );
+
+            lemma_updateConsensusInstanceValidityCheck(
+                                process.attestation_consensus_engine_state,
+                                new_attestation_slashing_db,
+                                process_mod.attestation_consensus_engine_state 
+                                );
+
+            assert process_mod.attestation_consensus_engine_state.att_slashing_db_hist.Keys
+                    == process.attestation_consensus_engine_state.att_slashing_db_hist.Keys 
+                            + process.attestation_consensus_engine_state.attestation_consensus_active_instances.Keys;
+
+            
+            assert inv5_body(process_mod);
+            assert inv26_body(process_mod);
+            assert inv28_body(process_mod);
+
+            lemma_inv28_f_check_for_next_queued_duty(process_mod, process');
+        }
+        else
+        {               
+            assert inv28_body(process);
+        }
+    } 
+
+    lemma lemma_inv29_add_block_to_bn(
+        s: DVCNodeState,
+        block: BeaconBlock,
+        s': DVCNodeState 
+    )
+    requires add_block_to_bn.requires(s, block)
+    requires s' == add_block_to_bn(s, block)    
+    requires inv29_body(s)
+    ensures inv29_body(s')
+    { }
+
+    lemma lemma_inv29_f_listen_for_attestation_shares(
+        process: DVCNodeState,
+        attestation_share: AttestationShare,
+        process': DVCNodeState
+    )
+    requires f_listen_for_attestation_shares.requires(process, attestation_share)
+    requires process' == f_listen_for_attestation_shares(process, attestation_share).state        
+    requires inv29_body(process)
+    ensures inv29_body(process')
+    { }
+
+    lemma lemma_inv29_f_start_next_duty(process: DVCNodeState, attestation_duty: AttestationDuty, process': DVCNodeState)
+    requires f_start_next_duty.requires(process, attestation_duty)
+    requires process' == f_start_next_duty(process, attestation_duty).state   
+    requires attestation_duty in process.all_rcvd_duties
+    requires inv29_body(process)
+    ensures inv29_body(process')
+    { } 
+
+    lemma lemma_inv29_f_resend_attestation_share(
+        process: DVCNodeState,
+        process': DVCNodeState)
+    requires f_resend_attestation_share.requires(process)
+    requires process' == f_resend_attestation_share(process).state        
+    requires inv29_body(process)
+    ensures inv29_body(process')
+    { } 
+
+    lemma lemma_inv29_f_check_for_next_queued_duty(
+        process: DVCNodeState,
+        process': DVCNodeState
+    )
+    requires f_check_for_next_queued_duty.requires(process)
+    requires process' == f_check_for_next_queued_duty(process).state    
+    requires inv5_body(process)
+    requires inv25_body(process)
+    requires inv29_body(process)
+    ensures inv29_body(process')
+    decreases process.attestation_duties_queue
+    {
+        if  && process.attestation_duties_queue != [] 
+            && (
+                || process.attestation_duties_queue[0].slot in process.future_att_consensus_instances_already_decided
+                || !process.current_attestation_duty.isPresent()
+            )    
+        {            
+                if process.attestation_duties_queue[0].slot in process.future_att_consensus_instances_already_decided.Keys 
+                {
+                    var queue_head := process.attestation_duties_queue[0];
+                    var new_attestation_slashing_db := f_update_attestation_slashing_db(process.attestation_slashing_db, process.future_att_consensus_instances_already_decided[queue_head.slot]);
+                    var process_mod := process.(
+                        attestation_duties_queue := process.attestation_duties_queue[1..],
+                        future_att_consensus_instances_already_decided := process.future_att_consensus_instances_already_decided - {queue_head.slot},
+                        attestation_slashing_db := new_attestation_slashing_db,
+                        attestation_consensus_engine_state := updateConsensusInstanceValidityCheck(
+                            process.attestation_consensus_engine_state,
+                            new_attestation_slashing_db
+                        )                        
+                    );
+
+                    lemma_updateConsensusInstanceValidityCheck(
+                                process.attestation_consensus_engine_state,
+                                new_attestation_slashing_db,
+                                process_mod.attestation_consensus_engine_state 
+                                );
+
+                    assert process_mod.attestation_consensus_engine_state.att_slashing_db_hist.Keys
+                                == process.attestation_consensus_engine_state.att_slashing_db_hist.Keys 
+                                        + process.attestation_consensus_engine_state.attestation_consensus_active_instances.Keys;
+
+                    assert inv25_body(process_mod);
+
+                    assert inv5_body(process_mod);
+                    assert inv29_body(process_mod);
+                    lemma_inv29_f_check_for_next_queued_duty(process_mod, process');
+                }
+                else
+                { 
+                    var process_mod := process.(
+                        attestation_duties_queue := process.attestation_duties_queue[1..]
+                    );     
+                    assert inv5_body(process_mod);
+                    assert inv29_body(process_mod);
+                    lemma_inv29_f_start_next_duty(process_mod, process.attestation_duties_queue[0], process');
+                }
+        }
+        else
+        { 
+            assert process'.all_rcvd_duties == process.all_rcvd_duties;
+        }
+    }
+
+    lemma lemma_inv29_f_att_consensus_decided(
+        process: DVCNodeState,
+        id: Slot,
+        decided_attestation_data: AttestationData, 
+        process': DVCNodeState
+    )
+    requires f_att_consensus_decided.requires(process, id, decided_attestation_data)
+    requires process' == f_att_consensus_decided(process, id, decided_attestation_data).state         
+    requires inv5_body(process)
+    requires inv25_body(process)
+    requires inv29_body(process)
+    ensures inv29_body(process')
+    {
+        
+        var local_current_attestation_duty := process.current_attestation_duty.safe_get();
+        var attestation_slashing_db := f_update_attestation_slashing_db(process.attestation_slashing_db, decided_attestation_data);
+
+        var fork_version := bn_get_fork_version(compute_start_slot_at_epoch(decided_attestation_data.target.epoch));
+        var attestation_signing_root := compute_attestation_signing_root(decided_attestation_data, fork_version);
+        var attestation_signature_share := rs_sign_attestation(decided_attestation_data, fork_version, attestation_signing_root, process.rs);
+        var attestation_with_signature_share := AttestationShare(
+                aggregation_bits := get_aggregation_bits(local_current_attestation_duty.validator_index),
+                data := decided_attestation_data, 
+                signature := attestation_signature_share
+            ); 
+
+        var new_attestation_consensus_engine_state := updateConsensusInstanceValidityCheck(
+                                                            process.attestation_consensus_engine_state,
+                                                            attestation_slashing_db
+                                                      );
+
+        var process_mod := 
+            process.(
+                current_attestation_duty := None,
+                attestation_shares_to_broadcast := process.attestation_shares_to_broadcast[local_current_attestation_duty.slot := attestation_with_signature_share],
+                attestation_slashing_db := attestation_slashing_db,
+                attestation_consensus_engine_state := new_attestation_consensus_engine_state
+            );
+    
+        lemma_updateConsensusInstanceValidityCheck(
+                                process.attestation_consensus_engine_state,
+                                attestation_slashing_db,
+                                process_mod.attestation_consensus_engine_state 
+                                );
+
+        assert process_mod.attestation_consensus_engine_state.att_slashing_db_hist.Keys
+                    == process.attestation_consensus_engine_state.att_slashing_db_hist.Keys 
+                            + process.attestation_consensus_engine_state.attestation_consensus_active_instances.Keys;
+
+
+        assert inv5_body(process_mod);
+        assert inv25_body(process_mod);
+
+        assert inv29_body(process_mod);
+
+        var ret_dvc := f_check_for_next_queued_duty(process_mod).state;
+        lemma_inv5_f_check_for_next_queued_duty(process_mod, ret_dvc);
+        assert inv5_body(ret_dvc);
+        
+        lemma_inv29_f_check_for_next_queued_duty(process_mod, ret_dvc);
+        assert inv29_body(ret_dvc);
+
+        assert process' == ret_dvc;        
+    }
+
+    lemma lemma_inv29_f_serve_attestation_duty(
+        process: DVCNodeState,
+        attestation_duty: AttestationDuty,
+        process': DVCNodeState
+    )  
+    requires f_serve_attestation_duty.requires(process, attestation_duty)
+    requires process' == f_serve_attestation_duty(process, attestation_duty).state
+    requires inv5_body(process)
+    requires inv25_body(process)
+    requires inv29_body(process)
+    ensures inv29_body(process')
+    {
+        var process_mod := process.(
+                attestation_duties_queue := process.attestation_duties_queue + [attestation_duty],
+                all_rcvd_duties := process.all_rcvd_duties + {attestation_duty}
+            );        
+
+        assert inv5_body(process_mod);
+        assert inv25_body(process_mod);
+        assert inv29_body(process_mod);
+        
+        lemma_inv29_f_check_for_next_queued_duty(process_mod, process');        
+    }
+
+    lemma lemma_inv29_f_listen_for_new_imported_blocks(
+        process: DVCNodeState,
+        block: BeaconBlock,
+        process': DVCNodeState
+    )
+    requires f_listen_for_new_imported_blocks.requires(process, block)
+    requires process' == f_listen_for_new_imported_blocks(process, block).state        
+    requires inv5_body(process)
+    requires inv25_body(process)
+    requires inv29_body(process)
+    ensures inv29_body(process')
+    {
+        var new_consensus_instances_already_decided := f_listen_for_new_imported_blocks_helper_1(process, block);
+
+        var att_consensus_instances_already_decided := process.future_att_consensus_instances_already_decided + new_consensus_instances_already_decided;
+
+        var future_att_consensus_instances_already_decided := 
+            f_listen_for_new_imported_blocks_helper_2(process, att_consensus_instances_already_decided);
+
+        var process :=
+                process.(
+                    future_att_consensus_instances_already_decided := future_att_consensus_instances_already_decided,
+                    attestation_consensus_engine_state := stopConsensusInstances(
+                                    process.attestation_consensus_engine_state,
+                                    att_consensus_instances_already_decided.Keys
+                    ),
+                    attestation_shares_to_broadcast := process.attestation_shares_to_broadcast - att_consensus_instances_already_decided.Keys,
+                    rcvd_attestation_shares := process.rcvd_attestation_shares - att_consensus_instances_already_decided.Keys                    
+                );    
+        
+        assert inv5_body(process);
+        assert inv25_body(process);
+        assert inv29_body(process);
+
+        if process.current_attestation_duty.isPresent() && process.current_attestation_duty.safe_get().slot in att_consensus_instances_already_decided
+        {
+            var decided_attestation_data := att_consensus_instances_already_decided[process.current_attestation_duty.safe_get().slot];
+            var new_attestation_slashing_db := f_update_attestation_slashing_db(process.attestation_slashing_db, decided_attestation_data);
+            var new_attestation_consensus_engine_state := updateConsensusInstanceValidityCheck(
+                                                            process.attestation_consensus_engine_state,
+                                                            new_attestation_slashing_db
+                                                          );  
+            var process_mod := process.(
+                current_attestation_duty := None,
+                attestation_slashing_db := new_attestation_slashing_db,
+                attestation_consensus_engine_state := new_attestation_consensus_engine_state
+            );
+
+            lemma_updateConsensusInstanceValidityCheck(
+                                process.attestation_consensus_engine_state,
+                                new_attestation_slashing_db,
+                                process_mod.attestation_consensus_engine_state 
+                                );
+
+            assert process_mod.attestation_consensus_engine_state.att_slashing_db_hist.Keys
+                    == process.attestation_consensus_engine_state.att_slashing_db_hist.Keys 
+                            + process.attestation_consensus_engine_state.attestation_consensus_active_instances.Keys;
+
+            
+            assert inv5_body(process_mod);
+            assert inv25_body(process_mod);
+            assert inv29_body(process_mod);
+
+            lemma_inv29_f_check_for_next_queued_duty(process_mod, process');
+        }
+        else
+        {               
+            assert inv29_body(process);
+        }
+    }   
+
+    lemma lemma_inv30_add_block_to_bn(
+        s: DVCNodeState,
+        block: BeaconBlock,
+        s': DVCNodeState 
+    )
+    requires add_block_to_bn.requires(s, block)
+    requires s' == add_block_to_bn(s, block)    
+    ensures s.attestation_slashing_db <= s'.attestation_slashing_db
+    { }
+
+    lemma lemma_inv30_f_listen_for_attestation_shares(
+        process: DVCNodeState,
+        attestation_share: AttestationShare,
+        process': DVCNodeState
+    )
+    requires f_listen_for_attestation_shares.requires(process, attestation_share)
+    requires process' == f_listen_for_attestation_shares(process, attestation_share).state        
+    ensures process.attestation_slashing_db <= process'.attestation_slashing_db    
+    { }
+
+    lemma lemma_inv30_f_start_next_duty(process: DVCNodeState, attestation_duty: AttestationDuty, process': DVCNodeState)
+    requires f_start_next_duty.requires(process, attestation_duty)
+    requires process' == f_start_next_duty(process, attestation_duty).state       
+    ensures process.attestation_slashing_db <= process'.attestation_slashing_db 
+    { } 
+
+    lemma lemma_inv30_f_resend_attestation_share(
+        process: DVCNodeState,
+        process': DVCNodeState)
+    requires f_resend_attestation_share.requires(process)
+    requires process' == f_resend_attestation_share(process).state        
+    ensures process.attestation_slashing_db <= process'.attestation_slashing_db     
+    { } 
+
+
+    lemma lemma_inv30_f_check_for_next_queued_duty(
+        process: DVCNodeState,
+        process': DVCNodeState
+    )
+    requires f_check_for_next_queued_duty.requires(process)
+    requires process' == f_check_for_next_queued_duty(process).state        
+    ensures process.attestation_slashing_db <= process'.attestation_slashing_db 
+    decreases process.attestation_duties_queue
+    {
+        if  && process.attestation_duties_queue != [] 
+            && (
+                || process.attestation_duties_queue[0].slot in process.future_att_consensus_instances_already_decided
+                || !process.current_attestation_duty.isPresent()
+            )    
+        {            
+                if process.attestation_duties_queue[0].slot in process.future_att_consensus_instances_already_decided.Keys 
+                {
+                    var queue_head := process.attestation_duties_queue[0];
+                    var new_attestation_slashing_db := f_update_attestation_slashing_db(process.attestation_slashing_db, process.future_att_consensus_instances_already_decided[queue_head.slot]);
+                    var process_mod := process.(
+                        attestation_duties_queue := process.attestation_duties_queue[1..],
+                        future_att_consensus_instances_already_decided := process.future_att_consensus_instances_already_decided - {queue_head.slot},
+                        attestation_slashing_db := new_attestation_slashing_db,
+                        attestation_consensus_engine_state := updateConsensusInstanceValidityCheck(
+                            process.attestation_consensus_engine_state,
+                            new_attestation_slashing_db
+                        )                        
+                    );
+
+                    assert process.attestation_slashing_db <= process_mod.attestation_slashing_db;
+                    
+                    lemma_inv30_f_check_for_next_queued_duty(process_mod, process');
+                }
+                else
+                { 
+                    var process_mod := process.(
+                        attestation_duties_queue := process.attestation_duties_queue[1..]
+                    );     
+                    assert process.attestation_slashing_db <= process_mod.attestation_slashing_db;
+                    lemma_inv30_f_start_next_duty(process_mod, process.attestation_duties_queue[0], process');
+                }
+        }
+        else
+        { 
+            assert process.attestation_slashing_db == process'.attestation_slashing_db;
+        }
+    }
+
+    lemma lemma_inv30_f_att_consensus_decided(
+        process: DVCNodeState,
+        id: Slot,
+        decided_attestation_data: AttestationData, 
+        process': DVCNodeState
+    )
+    requires f_att_consensus_decided.requires(process, id, decided_attestation_data)
+    requires process' == f_att_consensus_decided(process, id, decided_attestation_data).state         
+    ensures process.attestation_slashing_db <= process'.attestation_slashing_db
+    {
+        
+        var local_current_attestation_duty := process.current_attestation_duty.safe_get();
+        var attestation_slashing_db := f_update_attestation_slashing_db(process.attestation_slashing_db, decided_attestation_data);
+
+        var fork_version := bn_get_fork_version(compute_start_slot_at_epoch(decided_attestation_data.target.epoch));
+        var attestation_signing_root := compute_attestation_signing_root(decided_attestation_data, fork_version);
+        var attestation_signature_share := rs_sign_attestation(decided_attestation_data, fork_version, attestation_signing_root, process.rs);
+        var attestation_with_signature_share := AttestationShare(
+                aggregation_bits := get_aggregation_bits(local_current_attestation_duty.validator_index),
+                data := decided_attestation_data, 
+                signature := attestation_signature_share
+            ); 
+
+        var new_attestation_consensus_engine_state := updateConsensusInstanceValidityCheck(
+                                                            process.attestation_consensus_engine_state,
+                                                            attestation_slashing_db
+                                                      );
+
+        var process_mod := 
+            process.(
+                current_attestation_duty := None,
+                attestation_shares_to_broadcast := process.attestation_shares_to_broadcast[local_current_attestation_duty.slot := attestation_with_signature_share],
+                attestation_slashing_db := attestation_slashing_db,
+                attestation_consensus_engine_state := new_attestation_consensus_engine_state
+            );
+    
+        assert process.attestation_slashing_db <= process_mod.attestation_slashing_db;
+
+        var ret_dvc := f_check_for_next_queued_duty(process_mod).state;
+        
+        lemma_inv30_f_check_for_next_queued_duty(process_mod, ret_dvc);
+        
+        assert process' == ret_dvc;        
+    }
+
+    lemma lemma_inv30_f_serve_attestation_duty(
+        process: DVCNodeState,
+        attestation_duty: AttestationDuty,
+        process': DVCNodeState
+    )  
+    requires f_serve_attestation_duty.requires(process, attestation_duty)
+    requires process' == f_serve_attestation_duty(process, attestation_duty).state
+    ensures process.attestation_slashing_db <= process'.attestation_slashing_db
+    {
+        var process_mod := process.(
+                attestation_duties_queue := process.attestation_duties_queue + [attestation_duty],
+                all_rcvd_duties := process.all_rcvd_duties + {attestation_duty}
+            );        
+
+        assert process.attestation_slashing_db <= process_mod.attestation_slashing_db;
+
+        lemma_inv30_f_check_for_next_queued_duty(process_mod, process');        
+    }
+
+    lemma lemma_inv30_f_listen_for_new_imported_blocks(
+        process: DVCNodeState,
+        block: BeaconBlock,
+        process': DVCNodeState
+    )
+    requires f_listen_for_new_imported_blocks.requires(process, block)
+    requires process' == f_listen_for_new_imported_blocks(process, block).state   
+    ensures process.attestation_slashing_db <= process'.attestation_slashing_db     
+    {
+        var new_consensus_instances_already_decided := f_listen_for_new_imported_blocks_helper_1(process, block);
+
+        var att_consensus_instances_already_decided := process.future_att_consensus_instances_already_decided + new_consensus_instances_already_decided;
+
+        var future_att_consensus_instances_already_decided := 
+            f_listen_for_new_imported_blocks_helper_2(process, att_consensus_instances_already_decided);
+
+        var process :=
+                process.(
+                    future_att_consensus_instances_already_decided := future_att_consensus_instances_already_decided,
+                    attestation_consensus_engine_state := stopConsensusInstances(
+                                    process.attestation_consensus_engine_state,
+                                    att_consensus_instances_already_decided.Keys
+                    ),
+                    attestation_shares_to_broadcast := process.attestation_shares_to_broadcast - att_consensus_instances_already_decided.Keys,
+                    rcvd_attestation_shares := process.rcvd_attestation_shares - att_consensus_instances_already_decided.Keys                    
+                );    
+                
+
+        if process.current_attestation_duty.isPresent() && process.current_attestation_duty.safe_get().slot in att_consensus_instances_already_decided
+        {
+            var decided_attestation_data := att_consensus_instances_already_decided[process.current_attestation_duty.safe_get().slot];
+            var new_attestation_slashing_db := f_update_attestation_slashing_db(process.attestation_slashing_db, decided_attestation_data);
+            var new_attestation_consensus_engine_state := updateConsensusInstanceValidityCheck(
+                                                            process.attestation_consensus_engine_state,
+                                                            new_attestation_slashing_db
+                                                          );  
+            var process_mod := process.(
+                current_attestation_duty := None,
+                attestation_slashing_db := new_attestation_slashing_db,
+                attestation_consensus_engine_state := new_attestation_consensus_engine_state
+            );
+
+            
+
+            lemma_inv30_f_check_for_next_queued_duty(process_mod, process');
+        }
+        else
+        { }
+    } 
+
+    lemma lemma_inv30_dvn_next(
+        dvn: DVState,
+        event: DV.Event,
+        dvn': DVState
+    )    
+    requires NextEvent(dvn, event, dvn')  
+    ensures inv30(dvn, event, dvn')
+    {        
+        match event 
+        {
+            case HonestNodeTakingStep(node, nodeEvent, nodeOutputs) =>
+                var dvc := dvn.honest_nodes_states[node];
+                var dvc' := dvn'.honest_nodes_states[node];                
+                
+                match nodeEvent
+                {
+                    case ServeAttstationDuty(attestation_duty) =>   
+                        lemma_inv30_f_serve_attestation_duty(dvc, attestation_duty, dvc');
+                        
+                    case AttConsensusDecided(id, decided_attestation_data) => 
+                        lemma_inv30_f_att_consensus_decided(dvc, id, decided_attestation_data, dvc');
+                        
+                    case ReceviedAttesttionShare(attestation_share) =>                         
+                        lemma_inv30_f_listen_for_attestation_shares(dvc, attestation_share, dvc');
+                       
+                    case ImportedNewBlock(block) => 
+                        var dvc_mod := add_block_to_bn(dvc, block);
+                        lemma_inv30_add_block_to_bn(dvc, block, dvc_mod);
+                        lemma_inv30_f_listen_for_new_imported_blocks(dvc_mod, block, dvc');                        
+
+                    case ResendAttestationShares =>                                                                      
+
+                    case NoEvent => 
+                        
+                }
+                
+            case AdeversaryTakingStep(node, new_attestation_share_sent, messagesReceivedByTheNode) =>
+                
+        }   
+    }
+
+    lemma lemma_inv31_add_block_to_bn(
+        s: DVCNodeState,
+        block: BeaconBlock,
+        s': DVCNodeState 
+    )
+    requires add_block_to_bn.requires(s, block)
+    requires s' == add_block_to_bn(s, block)    
+    requires inv31_body(s)
+    ensures inv31_body(s')
+    { }
+
+    lemma lemma_inv31_f_listen_for_attestation_shares(
+        process: DVCNodeState,
+        attestation_share: AttestationShare,
+        process': DVCNodeState
+    )
+    requires f_listen_for_attestation_shares.requires(process, attestation_share)
+    requires process' == f_listen_for_attestation_shares(process, attestation_share).state        
+    requires inv31_body(process)
+    ensures inv31_body(process')
+    { }
+
+    lemma lemma_inv31_f_start_next_duty(process: DVCNodeState, attestation_duty: AttestationDuty, process': DVCNodeState)
+    requires f_start_next_duty.requires(process, attestation_duty)
+    requires process' == f_start_next_duty(process, attestation_duty).state   
+    requires attestation_duty in process.all_rcvd_duties
+    requires inv31_body(process)
+    ensures inv31_body(process')
+    { } 
+
+    lemma lemma_inv31_f_resend_attestation_share(
+        process: DVCNodeState,
+        process': DVCNodeState)
+    requires f_resend_attestation_share.requires(process)
+    requires process' == f_resend_attestation_share(process).state        
+    requires inv31_body(process)
+    ensures inv31_body(process')
+    { } 
+
+    
+
+    lemma lemma_inv31_f_check_for_next_queued_duty(
+        process: DVCNodeState,
+        process': DVCNodeState
+    )
+    requires f_check_for_next_queued_duty.requires(process)
+    requires process' == f_check_for_next_queued_duty(process).state    
+    requires inv5_body(process)
+    requires inv26_body(process)    
+    requires inv31_body(process)
+    ensures inv31_body(process')
+    decreases process.attestation_duties_queue
+    {
+        if  && process.attestation_duties_queue != [] 
+            && (
+                || process.attestation_duties_queue[0].slot in process.future_att_consensus_instances_already_decided
+                || !process.current_attestation_duty.isPresent()
+            )    
+        {            
+                if process.attestation_duties_queue[0].slot in process.future_att_consensus_instances_already_decided.Keys 
+                {
+                    var queue_head := process.attestation_duties_queue[0];
+                    var new_attestation_slashing_db := f_update_attestation_slashing_db(process.attestation_slashing_db, process.future_att_consensus_instances_already_decided[queue_head.slot]);
+                    assert process.attestation_slashing_db <= new_attestation_slashing_db;
+                    assert inv31_body_ces(process.attestation_consensus_engine_state, 
+                                          process.attestation_slashing_db);        
+
+
+                    forall s: Slot, vp: AttestationData -> bool, db: set<SlashingDBAttestation> |
+                            ( && s  in process.attestation_consensus_engine_state.att_slashing_db_hist.Keys
+                              && vp in process.attestation_consensus_engine_state.att_slashing_db_hist[s]
+                              && db in process.attestation_consensus_engine_state.att_slashing_db_hist[s][vp]
+                            )  
+                    ensures db <= new_attestation_slashing_db               
+                    {
+                        calc {
+                            db; 
+                            <=
+                            process.attestation_slashing_db;
+                            <=
+                            new_attestation_slashing_db;
+                        }                        
+                    }
+
+                    assert inv31_body_ces(process.attestation_consensus_engine_state, 
+                                          new_attestation_slashing_db);
+
+                    var process_mod := process.(
+                        attestation_duties_queue := process.attestation_duties_queue[1..],
+                        future_att_consensus_instances_already_decided := process.future_att_consensus_instances_already_decided - {queue_head.slot},
+                        attestation_slashing_db := new_attestation_slashing_db,
+                        attestation_consensus_engine_state := updateConsensusInstanceValidityCheck(
+                            process.attestation_consensus_engine_state,
+                            new_attestation_slashing_db
+                        )                        
+                    );
+                    assert process_mod.attestation_slashing_db <= new_attestation_slashing_db;                    
+                    assert inv26_body(process_mod);
+                    assert inv31_body_ces(process_mod.attestation_consensus_engine_state, 
+                                          new_attestation_slashing_db);
+
+                    assert inv5_body(process_mod);                    
+                    assert inv31_body(process_mod);
+                    lemma_inv31_f_check_for_next_queued_duty(process_mod, process');
+                }
+                else
+                { 
+                    var process_mod := process.(
+                        attestation_duties_queue := process.attestation_duties_queue[1..]
+                    );     
+                    assert inv5_body(process_mod);
+                    assert inv31_body(process_mod);
+                    lemma_inv31_f_start_next_duty(process_mod, process.attestation_duties_queue[0], process');
+                }
+        }
+        else
+        { 
+            assert inv31_body(process');
+        }
+    }
+
+    lemma lemma_inv31_f_att_consensus_decided(
+        process: DVCNodeState,
+        id: Slot,
+        decided_attestation_data: AttestationData, 
+        process': DVCNodeState
+    )
+    requires f_att_consensus_decided.requires(process, id, decided_attestation_data)
+    requires process' == f_att_consensus_decided(process, id, decided_attestation_data).state         
+    requires inv5_body(process)
+    requires inv26_body(process)
+    requires inv31_body(process)
+    ensures inv31_body(process')
+    {
+        
+        var local_current_attestation_duty := process.current_attestation_duty.safe_get();
+        var attestation_slashing_db := f_update_attestation_slashing_db(process.attestation_slashing_db, decided_attestation_data);
+        assert process.attestation_slashing_db <= attestation_slashing_db;
+        assert inv31_body_ces(process.attestation_consensus_engine_state, 
+                              process.attestation_slashing_db); 
+
+        forall s: Slot, vp: AttestationData -> bool, db: set<SlashingDBAttestation> |
+                            ( && s  in process.attestation_consensus_engine_state.att_slashing_db_hist.Keys
+                              && vp in process.attestation_consensus_engine_state.att_slashing_db_hist[s]
+                              && db in process.attestation_consensus_engine_state.att_slashing_db_hist[s][vp]
+                            )   
+        ensures db <= attestation_slashing_db               
+        {
+            calc {
+                db; 
+                <=
+                process.attestation_slashing_db;
+                <=
+                attestation_slashing_db;
+            }                        
+        }
+
+        assert inv31_body_ces(process.attestation_consensus_engine_state, 
+                              attestation_slashing_db);
+
+        var fork_version := bn_get_fork_version(compute_start_slot_at_epoch(decided_attestation_data.target.epoch));
+        var attestation_signing_root := compute_attestation_signing_root(decided_attestation_data, fork_version);
+        var attestation_signature_share := rs_sign_attestation(decided_attestation_data, fork_version, attestation_signing_root, process.rs);
+        var attestation_with_signature_share := AttestationShare(
+                aggregation_bits := get_aggregation_bits(local_current_attestation_duty.validator_index),
+                data := decided_attestation_data, 
+                signature := attestation_signature_share
+            ); 
+
+        var new_attestation_consensus_engine_state := updateConsensusInstanceValidityCheck(
+                                                            process.attestation_consensus_engine_state,
+                                                            attestation_slashing_db
+                                                      );
+
+        assert inv26_body(process);
+
+
+        lemma_inv31_updateConsensusInstanceValidityCheck(
+                                process.attestation_consensus_engine_state,
+                                attestation_slashing_db,
+                                new_attestation_consensus_engine_state
+                                );
+
+
+        assert inv31_body_ces(new_attestation_consensus_engine_state, attestation_slashing_db);
+
+        var process_mod := 
+            process.(
+                current_attestation_duty := None,
+                attestation_shares_to_broadcast := process.attestation_shares_to_broadcast[local_current_attestation_duty.slot := attestation_with_signature_share],
+                attestation_slashing_db := attestation_slashing_db,
+                attestation_consensus_engine_state := new_attestation_consensus_engine_state
+            );
+
+        assert inv31_body(process_mod);
+    
+        var ret_dvc := f_check_for_next_queued_duty(process_mod).state;
+        lemma_inv5_f_check_for_next_queued_duty(process_mod, ret_dvc);
+        assert inv5_body(ret_dvc);
+        
+        
+        lemma_inv31_f_check_for_next_queued_duty(process_mod, ret_dvc);
+        assert inv31_body(ret_dvc);
+
+        assert process' == ret_dvc;        
+    }
+
+    lemma lemma_inv31_f_serve_attestation_duty(
+        process: DVCNodeState,
+        attestation_duty: AttestationDuty,
+        process': DVCNodeState
+    )  
+    requires f_serve_attestation_duty.requires(process, attestation_duty)
+    requires process' == f_serve_attestation_duty(process, attestation_duty).state
+    requires inv5_body(process)
+    requires inv26_body(process)
+    requires inv31_body(process)
+    ensures inv31_body(process')
+    {
+        var process_mod := process.(
+                attestation_duties_queue := process.attestation_duties_queue + [attestation_duty],
+                all_rcvd_duties := process.all_rcvd_duties + {attestation_duty}
+            );        
+
+        assert inv5_body(process_mod);
+        assert inv26_body(process_mod);
+        assert inv31_body(process_mod);
+        
+        lemma_inv31_f_check_for_next_queued_duty(process_mod, process');        
+    }
+
+    lemma lemma_inv31_f_listen_for_new_imported_blocks(
+        process: DVCNodeState,
+        block: BeaconBlock,
+        process': DVCNodeState
+    )
+    requires f_listen_for_new_imported_blocks.requires(process, block)
+    requires process' == f_listen_for_new_imported_blocks(process, block).state        
+    requires inv5_body(process)
+    requires inv26_body(process)
+    requires inv31_body(process)
+    ensures inv31_body(process')
+    {
+        var new_consensus_instances_already_decided := f_listen_for_new_imported_blocks_helper_1(process, block);
+
+        var att_consensus_instances_already_decided := process.future_att_consensus_instances_already_decided + new_consensus_instances_already_decided;
+
+        var future_att_consensus_instances_already_decided := 
+            f_listen_for_new_imported_blocks_helper_2(process, att_consensus_instances_already_decided);
+
+        var process :=
+                process.(
+                    future_att_consensus_instances_already_decided := future_att_consensus_instances_already_decided,
+                    attestation_consensus_engine_state := stopConsensusInstances(
+                                    process.attestation_consensus_engine_state,
+                                    att_consensus_instances_already_decided.Keys
+                    ),
+                    attestation_shares_to_broadcast := process.attestation_shares_to_broadcast - att_consensus_instances_already_decided.Keys,
+                    rcvd_attestation_shares := process.rcvd_attestation_shares - att_consensus_instances_already_decided.Keys                    
+                );    
+        
+        assert inv5_body(process);
+        assert inv26_body(process);
+        assert inv31_body(process);
+
+        if process.current_attestation_duty.isPresent() && process.current_attestation_duty.safe_get().slot in att_consensus_instances_already_decided
+        {
+            var decided_attestation_data := att_consensus_instances_already_decided[process.current_attestation_duty.safe_get().slot];
+            var new_attestation_slashing_db := f_update_attestation_slashing_db(process.attestation_slashing_db, decided_attestation_data);
+
+            assert process.attestation_slashing_db <= new_attestation_slashing_db;
+            assert inv31_body_ces(process.attestation_consensus_engine_state, 
+                              process.attestation_slashing_db); 
+
+            forall s: Slot, vp: AttestationData -> bool, db: set<SlashingDBAttestation> |
+                            ( && s  in process.attestation_consensus_engine_state.att_slashing_db_hist.Keys
+                              && vp in process.attestation_consensus_engine_state.att_slashing_db_hist[s]
+                              && db in process.attestation_consensus_engine_state.att_slashing_db_hist[s][vp]
+                            )   
+            ensures db <= new_attestation_slashing_db               
+            {
+                calc {
+                    db; 
+                    <=
+                    process.attestation_slashing_db;
+                    <=
+                    new_attestation_slashing_db;
+                }                        
+            }
+
+            assert inv31_body_ces(process.attestation_consensus_engine_state, 
+                              new_attestation_slashing_db);
+
+            var new_attestation_consensus_engine_state := updateConsensusInstanceValidityCheck(
+                                                            process.attestation_consensus_engine_state,
+                                                            new_attestation_slashing_db
+                                                          );  
+            var process_mod := process.(
+                current_attestation_duty := None,
+                attestation_slashing_db := new_attestation_slashing_db,
+                attestation_consensus_engine_state := new_attestation_consensus_engine_state
+            );
+
+            lemma_updateConsensusInstanceValidityCheck(
+                                process.attestation_consensus_engine_state,
+                                new_attestation_slashing_db,
+                                process_mod.attestation_consensus_engine_state 
+                                );
+
+            assert process_mod.attestation_consensus_engine_state.att_slashing_db_hist.Keys
+                    == process.attestation_consensus_engine_state.att_slashing_db_hist.Keys 
+                            + process.attestation_consensus_engine_state.attestation_consensus_active_instances.Keys;
+
+            
+            assert inv5_body(process_mod);
+            assert inv26_body(process_mod);
+            assert inv31_body(process_mod);
+
+            lemma_inv31_f_check_for_next_queued_duty(process_mod, process');
+        }
+        else
+        {               
+            assert inv31_body(process);
+        }
+    }   
+    
+    lemma lemma_inv32_add_block_to_bn(
+        s: DVCNodeState,
+        block: BeaconBlock,
+        s': DVCNodeState 
+    )
+    requires add_block_to_bn.requires(s, block)
+    requires s' == add_block_to_bn(s, block)    
+    ensures inv32_body(s, s')
+    { }
+
+    lemma lemma_inv32_f_listen_for_attestation_shares(
+        process: DVCNodeState,
+        attestation_share: AttestationShare,
+        process': DVCNodeState
+    )
+    requires f_listen_for_attestation_shares.requires(process, attestation_share)
+    requires process' == f_listen_for_attestation_shares(process, attestation_share).state        
+    ensures inv32_body(process, process')
+    { }
+
+    lemma lemma_inv32_f_start_next_duty(process: DVCNodeState, attestation_duty: AttestationDuty, process': DVCNodeState)
+    requires f_start_next_duty.requires(process, attestation_duty)
+    requires process' == f_start_next_duty(process, attestation_duty).state       
+    ensures inv32_body(process, process')
+    { } 
+
+    lemma lemma_inv32_f_resend_attestation_share(
+        process: DVCNodeState,
+        process': DVCNodeState)
+    requires f_resend_attestation_share.requires(process)
+    requires process' == f_resend_attestation_share(process).state        
+    ensures inv32_body(process, process')     
+    { } 
+
+
+    lemma lemma_inv32_f_check_for_next_queued_duty(
+        process: DVCNodeState,
+        process': DVCNodeState
+    )
+    requires f_check_for_next_queued_duty.requires(process)
+    requires process' == f_check_for_next_queued_duty(process).state        
+    ensures inv32_body(process, process')
+    decreases process.attestation_duties_queue
+    {
+        if  && process.attestation_duties_queue != [] 
+            && (
+                || process.attestation_duties_queue[0].slot in process.future_att_consensus_instances_already_decided
+                || !process.current_attestation_duty.isPresent()
+            )    
+        {            
+                if process.attestation_duties_queue[0].slot in process.future_att_consensus_instances_already_decided.Keys 
+                {
+                    var queue_head := process.attestation_duties_queue[0];
+                    var new_attestation_slashing_db := f_update_attestation_slashing_db(process.attestation_slashing_db, process.future_att_consensus_instances_already_decided[queue_head.slot]);
+                    var process_mod := process.(
+                        attestation_duties_queue := process.attestation_duties_queue[1..],
+                        future_att_consensus_instances_already_decided := process.future_att_consensus_instances_already_decided - {queue_head.slot},
+                        attestation_slashing_db := new_attestation_slashing_db,
+                        attestation_consensus_engine_state := updateConsensusInstanceValidityCheck(
+                            process.attestation_consensus_engine_state,
+                            new_attestation_slashing_db
+                        )                        
+                    );
+
+                    assert process.attestation_slashing_db <= process_mod.attestation_slashing_db;
+                    
+                    lemma_inv32_f_check_for_next_queued_duty(process_mod, process');
+                }
+                else
+                { 
+                    var process_mod := process.(
+                        attestation_duties_queue := process.attestation_duties_queue[1..]
+                    );     
+                    assert process.attestation_slashing_db <= process_mod.attestation_slashing_db;
+                    lemma_inv32_f_start_next_duty(process_mod, process.attestation_duties_queue[0], process');
+                }
+        }
+        else
+        { 
+            assert process.attestation_slashing_db == process'.attestation_slashing_db;
+        }
+    }
+
+    lemma lemma_inv32_f_att_consensus_decided(
+        process: DVCNodeState,
+        id: Slot,
+        decided_attestation_data: AttestationData, 
+        process': DVCNodeState
+    )
+    requires f_att_consensus_decided.requires(process, id, decided_attestation_data)
+    requires process' == f_att_consensus_decided(process, id, decided_attestation_data).state         
+    ensures inv32_body(process, process')
+    {
+        
+        var local_current_attestation_duty := process.current_attestation_duty.safe_get();
+        var attestation_slashing_db := f_update_attestation_slashing_db(process.attestation_slashing_db, decided_attestation_data);
+
+        var fork_version := bn_get_fork_version(compute_start_slot_at_epoch(decided_attestation_data.target.epoch));
+        var attestation_signing_root := compute_attestation_signing_root(decided_attestation_data, fork_version);
+        var attestation_signature_share := rs_sign_attestation(decided_attestation_data, fork_version, attestation_signing_root, process.rs);
+        var attestation_with_signature_share := AttestationShare(
+                aggregation_bits := get_aggregation_bits(local_current_attestation_duty.validator_index),
+                data := decided_attestation_data, 
+                signature := attestation_signature_share
+            ); 
+
+        var new_attestation_consensus_engine_state := updateConsensusInstanceValidityCheck(
+                                                            process.attestation_consensus_engine_state,
+                                                            attestation_slashing_db
+                                                      );
+
+        var process_mod := 
+            process.(
+                current_attestation_duty := None,
+                attestation_shares_to_broadcast := process.attestation_shares_to_broadcast[local_current_attestation_duty.slot := attestation_with_signature_share],
+                attestation_slashing_db := attestation_slashing_db,
+                attestation_consensus_engine_state := new_attestation_consensus_engine_state
+            );
+    
+        assert process.attestation_slashing_db <= process_mod.attestation_slashing_db;
+
+        var ret_dvc := f_check_for_next_queued_duty(process_mod).state;
+        
+        lemma_inv32_f_check_for_next_queued_duty(process_mod, ret_dvc);
+        
+        assert process' == ret_dvc;        
+    }
+
+    lemma lemma_inv32_f_serve_attestation_duty(
+        process: DVCNodeState,
+        attestation_duty: AttestationDuty,
+        process': DVCNodeState
+    )  
+    requires f_serve_attestation_duty.requires(process, attestation_duty)
+    requires process' == f_serve_attestation_duty(process, attestation_duty).state
+    ensures inv32_body(process, process')
+    {
+        var process_mod := process.(
+                attestation_duties_queue := process.attestation_duties_queue + [attestation_duty],
+                all_rcvd_duties := process.all_rcvd_duties + {attestation_duty}
+            );        
+
+        assert process.attestation_slashing_db <= process_mod.attestation_slashing_db;
+
+        lemma_inv32_f_check_for_next_queued_duty(process_mod, process');        
+    }
+
+    lemma lemma_inv32_f_listen_for_new_imported_blocks(
+        process: DVCNodeState,
+        block: BeaconBlock,
+        process': DVCNodeState
+    )
+    requires f_listen_for_new_imported_blocks.requires(process, block)
+    requires process' == f_listen_for_new_imported_blocks(process, block).state   
+    ensures inv32_body(process, process')    
+    {
+        var new_consensus_instances_already_decided := f_listen_for_new_imported_blocks_helper_1(process, block);
+
+        var att_consensus_instances_already_decided := process.future_att_consensus_instances_already_decided + new_consensus_instances_already_decided;
+
+        var future_att_consensus_instances_already_decided := 
+            f_listen_for_new_imported_blocks_helper_2(process, att_consensus_instances_already_decided);
+
+        var process :=
+                process.(
+                    future_att_consensus_instances_already_decided := future_att_consensus_instances_already_decided,
+                    attestation_consensus_engine_state := stopConsensusInstances(
+                                    process.attestation_consensus_engine_state,
+                                    att_consensus_instances_already_decided.Keys
+                    ),
+                    attestation_shares_to_broadcast := process.attestation_shares_to_broadcast - att_consensus_instances_already_decided.Keys,
+                    rcvd_attestation_shares := process.rcvd_attestation_shares - att_consensus_instances_already_decided.Keys                    
+                );    
+                
+
+        if process.current_attestation_duty.isPresent() && process.current_attestation_duty.safe_get().slot in att_consensus_instances_already_decided
+        {
+            var decided_attestation_data := att_consensus_instances_already_decided[process.current_attestation_duty.safe_get().slot];
+            var new_attestation_slashing_db := f_update_attestation_slashing_db(process.attestation_slashing_db, decided_attestation_data);
+            var new_attestation_consensus_engine_state := updateConsensusInstanceValidityCheck(
+                                                            process.attestation_consensus_engine_state,
+                                                            new_attestation_slashing_db
+                                                          );  
+            var process_mod := process.(
+                current_attestation_duty := None,
+                attestation_slashing_db := new_attestation_slashing_db,
+                attestation_consensus_engine_state := new_attestation_consensus_engine_state
+            );
+
+            
+
+            lemma_inv32_f_check_for_next_queued_duty(process_mod, process');
+        }
+        else
+        { }
+    } 
+
+
+    /*
+    lemma lemma_inv33_add_block_to_bn(
+        s: DVCNodeState,
+        block: BeaconBlock,
+        s': DVCNodeState,
+        k: Slot
+    )
+    requires add_block_to_bn.requires(s, block)
+    requires s' == add_block_to_bn(s, block)    
+    requires inv33_body(s, k)
+    ensures inv33_body(s', k)
+    { }
+
+    lemma lemma_inv33_f_listen_for_attestation_shares(
+        process: DVCNodeState,
+        attestation_share: AttestationShare,
+        process': DVCNodeState,
+        k: Slot
+    )
+    requires f_listen_for_attestation_shares.requires(process, attestation_share)
+    requires process' == f_listen_for_attestation_shares(process, attestation_share).state        
+    requires inv33_body(process, k)
+    ensures inv33_body(process', k)
+    { }
+
+    lemma lemma_inv33_f_start_next_duty(
+                process: DVCNodeState, 
+                attestation_duty: AttestationDuty, 
+                process': DVCNodeState,
+                k: Slot)
+    requires f_start_next_duty.requires(process, attestation_duty)
+    requires process' == f_start_next_duty(process, attestation_duty).state   
+    requires attestation_duty in process.all_rcvd_duties
+    requires inv33_body(process, k)
+    ensures inv33_body(process', k)
+    { } 
+
+    lemma lemma_inv33_f_resend_attestation_share(
+        process: DVCNodeState,
+        process': DVCNodeState,
+        k: Slot)
+    requires f_resend_attestation_share.requires(process)
+    requires process' == f_resend_attestation_share(process).state        
+    requires inv33_body(process, k)
+    ensures inv33_body(process', k)
+    { } 
+
+    lemma lemma_inv33_f_check_for_next_queued_duty(
+        process: DVCNodeState,
+        process': DVCNodeState,
+        k: Slot
+    )
+    requires f_check_for_next_queued_duty.requires(process)
+    requires process' == f_check_for_next_queued_duty(process).state    
+    requires inv5_body(process)
+    requires inv25_body(process)
+    requires inv33_body(process, k)
+    ensures inv33_body(process', k)
+    decreases process.attestation_duties_queue
+    {
+        if  && process.attestation_duties_queue != [] 
+            && (
+                || process.attestation_duties_queue[0].slot in process.future_att_consensus_instances_already_decided
+                || !process.current_attestation_duty.isPresent()
+            )    
+        {            
+                if process.attestation_duties_queue[0].slot in process.future_att_consensus_instances_already_decided.Keys 
+                {
+                    var queue_head := process.attestation_duties_queue[0];
+                    var new_attestation_slashing_db := f_update_attestation_slashing_db(process.attestation_slashing_db, process.future_att_consensus_instances_already_decided[queue_head.slot]);
+                    var process_mod := process.(
+                        attestation_duties_queue := process.attestation_duties_queue[1..],
+                        future_att_consensus_instances_already_decided := process.future_att_consensus_instances_already_decided - {queue_head.slot},
+                        attestation_slashing_db := new_attestation_slashing_db,
+                        attestation_consensus_engine_state := updateConsensusInstanceValidityCheck(
+                            process.attestation_consensus_engine_state,
+                            new_attestation_slashing_db
+                        )                        
+                    );
+
+                    lemma_updateConsensusInstanceValidityCheck(
+                                process.attestation_consensus_engine_state,
+                                new_attestation_slashing_db,
+                                process_mod.attestation_consensus_engine_state 
+                                );
+
+                    assert process_mod.attestation_consensus_engine_state.att_slashing_db_hist.Keys
+                                == process.attestation_consensus_engine_state.att_slashing_db_hist.Keys 
+                                        + process.attestation_consensus_engine_state.attestation_consensus_active_instances.Keys;
+
+                    assert inv25_body(process_mod);
+
+                    assert inv5_body(process_mod);
+                    assert inv33_body(process_mod, k);
+                    lemma_inv33_f_check_for_next_queued_duty(process_mod, process', k);
+                }
+                else
+                { 
+                    var process_mod := process.(
+                        attestation_duties_queue := process.attestation_duties_queue[1..]
+                    );     
+                    assert inv5_body(process_mod);
+                    assert inv33_body(process_mod, k);
+                    lemma_inv33_f_start_next_duty(process_mod, process.attestation_duties_queue[0], process', k);
+                }
+        }
+        else
+        { 
+            assert process'.all_rcvd_duties == process.all_rcvd_duties;
+        }
+    }
+
+    lemma lemma_inv33_f_att_consensus_decided(
+        process: DVCNodeState,
+        id: Slot,
+        decided_attestation_data: AttestationData, 
+        process': DVCNodeState,
+        k: Slot
+    )
+    requires f_att_consensus_decided.requires(process, id, decided_attestation_data)
+    requires process' == f_att_consensus_decided(process, id, decided_attestation_data).state         
+    requires inv5_body(process)
+    requires inv25_body(process)
+    requires inv33_body(process, k)
+    ensures inv33_body(process', k)
+    {
+        
+        var local_current_attestation_duty := process.current_attestation_duty.safe_get();
+        var attestation_slashing_db := f_update_attestation_slashing_db(process.attestation_slashing_db, decided_attestation_data);
+
+        var fork_version := bn_get_fork_version(compute_start_slot_at_epoch(decided_attestation_data.target.epoch));
+        var attestation_signing_root := compute_attestation_signing_root(decided_attestation_data, fork_version);
+        var attestation_signature_share := rs_sign_attestation(decided_attestation_data, fork_version, attestation_signing_root, process.rs);
+        var attestation_with_signature_share := AttestationShare(
+                aggregation_bits := get_aggregation_bits(local_current_attestation_duty.validator_index),
+                data := decided_attestation_data, 
+                signature := attestation_signature_share
+            ); 
+
+        var new_attestation_consensus_engine_state := updateConsensusInstanceValidityCheck(
+                                                            process.attestation_consensus_engine_state,
+                                                            attestation_slashing_db
+                                                      );
+
+        var process_mod := 
+            process.(
+                current_attestation_duty := None,
+                attestation_shares_to_broadcast := process.attestation_shares_to_broadcast[local_current_attestation_duty.slot := attestation_with_signature_share],
+                attestation_slashing_db := attestation_slashing_db,
+                attestation_consensus_engine_state := new_attestation_consensus_engine_state
+            );
+    
+        lemma_updateConsensusInstanceValidityCheck(
+                                process.attestation_consensus_engine_state,
+                                attestation_slashing_db,
+                                process_mod.attestation_consensus_engine_state 
+                                );
+
+        assert process_mod.attestation_consensus_engine_state.att_slashing_db_hist.Keys
+                    == process.attestation_consensus_engine_state.att_slashing_db_hist.Keys 
+                            + process.attestation_consensus_engine_state.attestation_consensus_active_instances.Keys;
+
+
+        assert inv5_body(process_mod);
+        assert inv25_body(process_mod);
+
+        assert inv33_body(process_mod, k);
+
+        var ret_dvc := f_check_for_next_queued_duty(process_mod).state;
+        lemma_inv5_f_check_for_next_queued_duty(process_mod, ret_dvc);
+        assert inv5_body(ret_dvc);
+        
+        lemma_inv33_f_check_for_next_queued_duty(process_mod, ret_dvc, k);
+        assert inv33_body(ret_dvc, k);
+
+        assert process' == ret_dvc;        
+    }
+
+    lemma lemma_inv33_f_serve_attestation_duty(
+        process: DVCNodeState,
+        attestation_duty: AttestationDuty,
+        process': DVCNodeState,
+        k: Slot
+    )  
+    requires f_serve_attestation_duty.requires(process, attestation_duty)
+    requires process' == f_serve_attestation_duty(process, attestation_duty).state
+    requires inv5_body(process)
+    requires inv25_body(process)
+    requires inv33_body(process, k)
+    ensures inv33_body(process', k)
+    {
+        var process_mod := process.(
+                attestation_duties_queue := process.attestation_duties_queue + [attestation_duty],
+                all_rcvd_duties := process.all_rcvd_duties + {attestation_duty}
+            );        
+
+        assert inv5_body(process_mod);
+        assert inv25_body(process_mod);
+        assert inv33_body(process_mod, k);
+        
+        lemma_inv33_f_check_for_next_queued_duty(process_mod, process', k);        
+    }
+
+    lemma lemma_inv33_f_listen_for_new_imported_blocks(
+        process: DVCNodeState,
+        block: BeaconBlock,
+        process': DVCNodeState,
+        k: Slot
+    )
+    requires f_listen_for_new_imported_blocks.requires(process, block)
+    requires process' == f_listen_for_new_imported_blocks(process, block).state        
+    requires inv5_body(process)
+    requires inv25_body(process)
+    requires inv33_body(process, k)
+    ensures inv33_body(process', k)
+    {
+        var new_consensus_instances_already_decided := f_listen_for_new_imported_blocks_helper_1(process, block);
+
+        var att_consensus_instances_already_decided := process.future_att_consensus_instances_already_decided + new_consensus_instances_already_decided;
+
+        var future_att_consensus_instances_already_decided := 
+            f_listen_for_new_imported_blocks_helper_2(process, att_consensus_instances_already_decided);
+
+        var process :=
+                process.(
+                    future_att_consensus_instances_already_decided := future_att_consensus_instances_already_decided,
+                    attestation_consensus_engine_state := stopConsensusInstances(
+                                    process.attestation_consensus_engine_state,
+                                    att_consensus_instances_already_decided.Keys
+                    ),
+                    attestation_shares_to_broadcast := process.attestation_shares_to_broadcast - att_consensus_instances_already_decided.Keys,
+                    rcvd_attestation_shares := process.rcvd_attestation_shares - att_consensus_instances_already_decided.Keys                    
+                );    
+        
+        assert inv5_body(process);
+        assert inv25_body(process);
+        assert inv33_body(process, k);
+
+        if process.current_attestation_duty.isPresent() && process.current_attestation_duty.safe_get().slot in att_consensus_instances_already_decided
+        {
+            var decided_attestation_data := att_consensus_instances_already_decided[process.current_attestation_duty.safe_get().slot];
+            var new_attestation_slashing_db := f_update_attestation_slashing_db(process.attestation_slashing_db, decided_attestation_data);
+            var new_attestation_consensus_engine_state := updateConsensusInstanceValidityCheck(
+                                                            process.attestation_consensus_engine_state,
+                                                            new_attestation_slashing_db
+                                                          );  
+            var process_mod := process.(
+                current_attestation_duty := None,
+                attestation_slashing_db := new_attestation_slashing_db,
+                attestation_consensus_engine_state := new_attestation_consensus_engine_state
+            );
+
+            lemma_updateConsensusInstanceValidityCheck(
+                                process.attestation_consensus_engine_state,
+                                new_attestation_slashing_db,
+                                process_mod.attestation_consensus_engine_state 
+                                );
+
+            assert process_mod.attestation_consensus_engine_state.att_slashing_db_hist.Keys
+                    == process.attestation_consensus_engine_state.att_slashing_db_hist.Keys 
+                            + process.attestation_consensus_engine_state.attestation_consensus_active_instances.Keys;
+
+            
+            assert inv5_body(process_mod);
+            assert inv25_body(process_mod);
+            assert inv33_body(process_mod, k);
+
+            lemma_inv33_f_check_for_next_queued_duty(process_mod, process', k);
+        }
+        else
+        {               
+            assert inv33_body(process, k);
+        }
+    }
+    */
+}
