src/dvspec/dafny/att_spec_proofs/incomplete_proofs.dfy
@@ -5,12 +5,13 @@ include "../specification/network.dfy"
 include "../specification/dvn.dfy"
 include "../att_spec_proofs/inv.dfy"
 include "../att_spec_proofs/assump.dfy"
-include "../att_spec_proofs/fnc_inv.dfy"
+include "../att_spec_proofs/fnc_invs_1_26.dfy"
 include "../att_spec_proofs/helper_sets_lemmas.dfy"
 include "../att_spec_proofs/dvn_next_invs_1_7.dfy"
 include "../att_spec_proofs/dvn_next_invs_8_18.dfy"
-include "../att_spec_proofs/dvn_next_invs_19.dfy"
-
+include "../att_spec_proofs/dvn_next_invs_19_26.dfy"
+include "../att_spec_proofs/common_proofs.dfy"
+include "../att_spec_proofs/fnc_invs_27.dfy"
 
 module Incomplete_Proofs 
 {
@@ -24,15 +25,221 @@ module Incomplete_Proofs
     import opened Helper_Sets_Lemmas
     import opened DVN_Next_Invs_1_7
     import opened DVN_Next_Invs_8_18
-    import opened DVN_Next_Invs_19
-    import opened Fnc_Inv    
+    import opened DVN_Next_Invs_19_26
+    import opened Fnc_Invs_1_26    
+    import opened Fnc_Invs_27
+    import opened Common_Proofs
+    
+
+    lemma {:axiom} axiom_inv33(dvn: DVState)    
+    ensures inv33(dvn)
+
+    
+
+ 
+
+    
+
+ 
+    lemma lemma_inv33_ServeAttstationDuty(
+        dvn: DVState,        
+        event: DV.Event,
+        dvn': DVState
+    )    
+    requires NextEvent(dvn, event, dvn')  
+    requires event.HonestNodeTakingStep?
+    requires event.event.ServeAttstationDuty?
+    requires inv5(dvn)
+    requires inv25(dvn)
+    requires inv33(dvn)  
+    // ensures inv33(dvn')
+    {        
+
+        match event 
+        {
+            case HonestNodeTakingStep(node, nodeEvent, nodeOutputs) =>
+                var dvc := dvn.honest_nodes_states[node];
+                var dvc' := dvn'.honest_nodes_states[node];                
+                
+                match nodeEvent
+                {
+                    case ServeAttstationDuty(attestation_duty) =>   
+                        forall hn: BLSPubkey | is_honest_node(dvn, hn)                             
+                        {
+                            
+                            if hn == node
+                            {
+                                assert && dvc == dvn.honest_nodes_states[hn]
+                                       && dvc' == dvn'.honest_nodes_states[hn];  
+
+                                forall k: Slot | k in dvn'.consensus_on_attestation_data
+                                {
+                                    if hn in dvn'.consensus_on_attestation_data[k].honest_nodes_validity_functions.Keys
+                                    {
+                                        
+                                    }
+                                    else
+                                    {
+                                    
+                                    }                                
+                                }
+                            }
+                            else
+                            {
+                                calc {
+                                    dvn.honest_nodes_states[hn];
+                                    ==
+                                    dvn'.honest_nodes_states[hn];                                      
+                                } 
+
+                                lemma_inv30_dvn_next(dvn, event, dvn');
+                                assert inv30_body(dvn.honest_nodes_states[hn], dvn'.honest_nodes_states[hn]);
+
+                                forall s: Slot | s in dvn'.consensus_on_attestation_data.Keys
+                                {
+                                    assert 
+                                    hn in dvn'.consensus_on_attestation_data[s].honest_nodes_validity_functions.Keys
+                                    ==>
+                                    hn in dvn.consensus_on_attestation_data[s].honest_nodes_validity_functions.Keys;
+                                } 
+
+                                forall s: Slot |
+                                     hn in dvn'.consensus_on_attestation_data[s].honest_nodes_validity_functions.Keys
+                                // ensures
+                                //    s in dvn'.honest_nodes_states[hn].attestation_consensus_engine_state.att_slashing_db_hist.Keys
+                                {
+                                    assert hn in dvn.consensus_on_attestation_data[s].honest_nodes_validity_functions.Keys;
+                                    assert dvn.consensus_on_attestation_data[s].honest_nodes_validity_functions[hn]
+                                             == dvn'.consensus_on_attestation_data[s].honest_nodes_validity_functions[hn];
+                                }
+                                
+
+                            
+                            }
+                        }
+                }
+        }
+    }
+
+/*
+    lemma lemma_inv33_dvn_next(
+        dvn: DVState,
+        event: DV.Event,
+        dvn': DVState
+    )    
+    requires NextEvent(dvn, event, dvn')  
+    requires inv5(dvn)
+    requires inv25(dvn)
+    requires inv33(dvn)  
+    // ensures inv33(dvn')
+    {        
+        match event 
+        {
+            case HonestNodeTakingStep(node, nodeEvent, nodeOutputs) =>
+                var dvc := dvn.honest_nodes_states[node];
+                var dvc' := dvn'.honest_nodes_states[node];                
+                
+                match nodeEvent
+                {
+                    case ServeAttstationDuty(attestation_duty) =>   
+                        forall hn: BLSPubkey, s: Slot | is_honest_node(dvn, hn)                             
+                        // ensures inv33_body(dvn'.honest_nodes_states[hn], s);
+                        {
+                            if hn in dvn.consensus_on_attestation_data[s].honest_nodes_validity_functions.Keys
+                            {
+                                if hn == node 
+                                {
+                                    assert inv5_body(dvn.honest_nodes_states[hn]);
+                                    assert inv25_body(dvn.honest_nodes_states[hn]);
+                                    assert inv33_body(dvn.honest_nodes_states[hn], s);
+                                    lemma_inv33_f_serve_attestation_duty(
+                                        dvn.honest_nodes_states[hn], 
+                                        attestation_duty, 
+                                        dvn'.honest_nodes_states[hn], 
+                                        s);
+                                    assert inv33_body(dvn'.honest_nodes_states[hn], s);
+                                }
+                                else
+                                {
+                                    assert dvn.honest_nodes_states[hn] == dvn'.honest_nodes_states[hn];
+                                    assert inv33_body(dvn'.honest_nodes_states[hn], s);
+                                }
+
+                                
+                            }
+                            else
+                            {
+                                assert hn !in dvn.consensus_on_attestation_data[s].honest_nodes_validity_functions.Keys;
+                            }
+                        }
+                        
+
+                    case AttConsensusDecided(id, decided_attestation_data) => 
+                    /*
+                        forall hn: BLSPubkey, s: Slot | 
+                            && is_honest_node(dvn, hn) 
+                            && hn in dvn.consensus_on_attestation_data[s].honest_nodes_validity_functions.Keys
+                        ensures inv33_body(dvn'.honest_nodes_states[hn], s);
+                        {
+                            if hn == node 
+                            {
+                                assert inv5_body(dvc);
+                                assert inv25_body(dvc);
+                                assert inv33_body(dvc, s);
+                                lemma_inv33_f_serve_attestation_duty(dvc, attestation_duty, dvc', s);
+                                assert inv33_body(dvc', s);
+                            }
+                            else
+                            {
+                                assert dvn.honest_nodes_states[hn] == dvn'.honest_nodes_states[hn];
+                                assert inv33_body(dvn'.honest_nodes_states[hn], s);
+                            }
+                        }
+*/
+                        // lemma_inv33_f_att_consensus_decided(dvc, id, decided_attestation_data, dvc');
+                        // assert inv33_body(dvc');
+                        axiom_inv33(dvn');
+                        
+                    case ReceviedAttesttionShare(attestation_share) =>                         
+                        // lemma_inv33_f_listen_for_attestation_shares(dvc, attestation_share, dvc');
+                        // assert inv33_body(dvc');
+                       axiom_inv33(dvn');
+
+                    case ImportedNewBlock(block) => 
+                    /*
+                        var dvc_mod := add_block_to_bn(dvc, block);
+                        lemma_inv5_add_block_to_bn(dvc, block, dvc_mod);
+                        assert inv5_body(dvc_mod);
+                        lemma_inv33_add_block_to_bn(dvc, block, dvc_mod);
+                        assert inv33_body(dvc_mod);
+                        lemma_inv33_f_listen_for_new_imported_blocks(dvc_mod, block, dvc');                        
+                        assert inv33_body(dvc');
+*/
+                        axiom_inv33(dvn');
+
+                    case ResendAttestationShares =>                                                                      
+
+                    case NoEvent => 
+                        
+                }
+                
+            case AdeversaryTakingStep(node, new_attestation_share_sent, messagesReceivedByTheNode) =>
+                
+        }   
+    }  
+    
+
+
+    
+*/
+    
+
+    
     
     
 
-    lemma {:axiom} axiom_inv26(dvn: DVState)    
-    ensures inv26(dvn)
-
     
+
     
     
 
